going to try brute force termination instead

theories/Logic/fol.v
@@ -23,48 +23,40 @@ Import ListNotations.
 (*Language*)
 Inductive nvec : nat -> Type :=
 | Null : nvec 0
-| New : forall (i : nat), nat -> nvec i -> nvec (S i).
+| New : forall {m : nat}, nat -> nvec m -> nvec (S m).
 
-Inductive predicate {n : nat} : nvec n -> Type :=
-| Nullary : forall (i : nat) (pf : n = 0), predicate (eq_rect _ _ Null _ (eq_sym pf))
-| Succary : forall {m : nat} {vec : nvec m} (i : nat) (v : ivar) (prd : predicate vec) (pf : n = S m), predicate (eq_rect _ _ (New m v vec) _ (eq_sym pf))
-| Var : forall {vec : nvec n} (i : nat), predicate vec.
+Inductive predicate : nat -> Type :=
+| Nullary : forall (i : nat), predicate 0
+| Succary : forall {m : nat} (i : nat) (prd : predicate m), @predicate (S m)
+| Var : forall {n : nat} (i : nat), predicate n.
 
-Fixpoint pure_predicate {n : nat} {vec : nvec n} (pn : predicate vec) : bool :=
+Fixpoint pure_predicate {n : nat} (pn : predicate n) : bool :=
 match pn with
-| Nullary _ _ => true
-| Succary _ _ pn' _ => pure_predicate pn'
+| Nullary _ => true
+| Succary _ pn' => pure_predicate pn'
 | Var _ => false
 end.
-
-(*
-Inductive predicate : nat -> Type :=
-| Nullary : forall (n : nat), predicate 0
-| Succary : forall {i : nat} (n : nat) (v : ivar) (prd : predicate i), predicate (S i).
-*)
 
 Inductive formula : Type :=
 | fal : formula
 | equ : ivar -> ivar -> formula
 | imp : formula -> formula -> formula
-| univ : ivar -> formula -> formula
+| univ : formula -> formula
 | bnd : ovar -> ovar -> formula -> formula
-| prd : forall {n : nat} {vec : nvec n} (pn : predicate vec), pure_predicate pn = true -> formula.
+| prd : forall {n : nat} (vec : nvec n) (pn : predicate n), pure_predicate pn = true -> formula.
 (*
 | mu : forall n, (predicate n) -> formula -> formula
 | muk : forall n, (predicate n) -> ordinal -> formula -> formula.
 *)
-
-
 
 Fixpoint num_conn (A : formula) : ordinal :=
 match A with
 | fal => cast Zero
 | equ v1 v2 => cast Zero
 | imp B C => oadd (oadd (num_conn B) (num_conn C)) (cast (nat_ord 1))
-| univ v B => oadd (num_conn B) (cast (nat_ord 1))
+| univ B => oadd (num_conn B) (cast (nat_ord 1))
 | bnd o1 o2 B => oadd (num_conn B) (cast (nat_ord 1))
-| prd pn pure => cast Zero
+| prd vec pn pure => cast Zero
 end.
 
 Fixpoint vars_in (a : formula) : list ovar :=
@@ -72,28 +64,25 @@ match a with
 | fal => []
 | equ v1 v2 => []
 | imp B C => (vars_in B) ++ (vars_in C)
-| univ v B => (vars_in B)
+| univ B => (vars_in B)
 | bnd o1 o2 B => o2 :: remove nat_eq_dec o1 (vars_in B)
-| prd pn pure => []
+| prd vec pn pure => []
 end.
 
 Fixpoint nvec_eqb {n1 n2 : nat} (vec1 : nvec n1) (vec2 : nvec n2) : bool :=
 match vec1, vec2 with
 | Null, Null => true (*nat_eqb m1 m2*)
-| New _ m1 vec1', New _ m2 vec2' => nat_eqb m1 m2 && nvec_eqb vec1' vec2'
+| New m1 vec1', New m2 vec2' => nat_eqb m1 m2 && nvec_eqb vec1' vec2'
 | _, _ => false
 end.
 
-Fixpoint prd_eqb {n1 n2 : nat} {vec1 : nvec n1} {vec2 : nvec n2} (pn1 : predicate vec1) (pn2 : predicate vec2) : bool :=
+Fixpoint prd_eqb {n1 n2 : nat} (pn1 : predicate n1) (pn2 : predicate n2) : bool :=
 match nat_eqb n1 n2 with
-| true => match nvec_eqb vec1 vec2 with
-    | true => match pn1, pn2 with
-        | Nullary i1 _, Nullary i2 _ => nat_eqb i1 i2
-        | Succary i1 v1 pn1' _, Succary i2 v2 pn2' _  => nat_eqb i1 i2 && nat_eqb v1 v2 && prd_eqb pn1' pn2'
-        | Var i1, Var i2 => nat_eqb i1 i2
-        | _ , _ => false
-        end
-    | false => false
+| true => match pn1, pn2 with
+    | Nullary i1, Nullary i2 => nat_eqb i1 i2
+    | Succary i1 pn1', Succary i2 pn2'  => nat_eqb i1 i2 && prd_eqb pn1' pn2'
+    | Var i1, Var i2 => nat_eqb i1 i2
+    | _ , _ => false
     end
 | false => false
 end.
@@ -103,10 +92,116 @@ match A1, A2 with
 | fal, fal => true
 | equ v1 v2, equ v3 v4 => nat_eqb v1 v3 && nat_eqb v2 v4
 | imp B1 C1, imp B2 C2 => form_eqb B1 B2 && form_eqb C1 C2
-| univ v1 B1, univ v2 B2 => nat_eqb v1 v2 && form_eqb B1 B2
+| univ B1, univ B2 => form_eqb B1 B2
 | bnd o1 o2 B1, bnd o3 o4 B2 => nat_eqb o1 o3 && nat_eqb o2 o4 && form_eqb B1 B2
-| prd pn1 _, prd pn2 _ => prd_eqb pn1 pn2
+| prd vec1 pn1 _, prd vec2 pn2 _ => nvec_eqb vec1 vec2 && prd_eqb pn1 pn2
 | _, _ => false
+end.
+
+(*
+Fixpoint in_vecb {n : nat} (vec : nvec n) (i : ivar) : bool :=
+match vec with
+| Null => false
+| New v vec' => nat_eqb v i || in_vecb vec' i
+end.
+
+Fixpoint free_var (phi : formula) (i : ivar) : bool :=
+match phi with
+| fal => false
+| equ v1 v2 => nat_eqb v1 i || nat_eqb v2 i
+| imp B C => free_var B i || free_var C i
+| univ B => match i with
+    | 0 => false
+    | S n => free_var B n
+    end
+| bnd o1 o2 B => free_var B i
+| prd vec pn pure => in_vecb vec i
+end.
+*)
+
+Fixpoint form_depth (phi : formula) : nat :=
+match phi with
+| fal => 0
+| equ v1 v2 => 0
+| imp B C => max (form_depth B) (form_depth C)
+| univ B => S (form_depth B)
+| bnd o1 o2 B => form_depth B
+| prd vec pn pure => 0
+end.
+
+Fixpoint vec_map {n : nat} (F : nat -> nat) (vec : nvec n) : nvec n :=
+match vec with
+| Null => Null
+| New v vec' => New (F v) (vec_map F vec')
+end.
+
+(*
+Fixpoint shift_subst (A : formula) (i1 i2 : ivar) : formula :=
+match A with
+| fal => fal
+| equ v1 v2 =>
+    match nat_semiconnex_type v1 i1, nat_semiconnex_type v2 i1 with
+    | inl (inl GT1), inl (inl GT2) => equ (pred v1) (pred v2)
+    | inl (inl GT1), inl (inr EQ2) => equ (pred v1) (v2 + i2)
+    | inl (inl GT1), inr LT2 => equ (pred v1) v2
+    | inl (inr EQ1), inl (inl GT2) => equ (v1 + i2) (pred v2)
+    | inl (inr EQ1), inl (inr EQ2) => equ (v1 + i2) (v2 + i2)
+    | inl (inr EQ1), inr LT2 => equ (v1 + i2) v2
+    | inr LT1, inl (inl GT2) => equ v1 (pred v2)
+    | inr LT1, inl (inr EQ2) => equ v1 (v2 + i2)
+    | inr LT1, inr LT2 => equ v1 v2
+    end
+| imp B C => imp (shift_subst B i1 i2) (shift_subst C i1 i2) 
+| univ B => univ (shift_subst B (S i1) i2)
+| bnd o1 o2 B => bnd o1 o2 (shift_subst B i1 i2)
+| prd vec pn pure =>
+    prd
+    (vec_map (fun n => match nat_semiconnex_type n i1 with
+              | inl (inl GT) => (pred n)
+              | inl (inr EQ) => (n + i2)
+              | inr LT => n
+              end) vec)
+    pn pure
+end.
+
+Lemma shift_subst_lemma :
+    forall (phi : formula) (i1 j1 i2 i3 : ivar),
+        shift_subst (shift_subst A i1 i2) (i1 + j1) i3 = shift_subst (shift_subst A (S (i1 + j1)) i3) i1 (i2)
+*)
+
+Fixpoint shift_substitution (A : formula) (i1 i2 : ivar) : formula :=
+match A with
+| fal => fal
+| equ v1 v2 => match nat_eqb v1 i1, nat_eqb v2 i1 with
+    | true, true => equ (v1 + i2) (v2 + i2)
+    | true, false => equ (v1 + i2) v2
+    | false, true => equ v1 (v2 + i2)
+    | false, false => equ v1 v2
+    end
+| imp B C => imp (shift_substitution B i1 i2) (shift_substitution C i1 i2)
+| univ B => univ (shift_substitution B (S i1) i2)
+| bnd o1 o2 B => bnd o1 o2 (shift_substitution B i1 i2)
+| prd vec pn pure => prd (vec_map (fun n => if nat_eqb n i1 then n + i2 else n) vec) pn pure
+end.
+
+
+Fixpoint substitution_depth (A : formula) (depth : nat) (i1 i2 : ivar) : formula :=
+match A with
+| fal => fal
+| equ v1 v2 => match nat_eqb v1 i1, nat_eqb v2 i1 with
+    | true, true => equ i2 i2
+    | true, false => equ i2 v2
+    | false, true => equ v1 i2
+    | false, false => equ v1 v2
+    end
+| imp B C => imp (substitution_depth B depth i1 i2) (substitution_depth C depth i1 i2)
+| univ B =>
+    (match nat_ltb depth i1, nat_ltb depth i2 with
+    | true, true => univ (substitution_depth B (S depth) i1 i2)
+    | _, _ => A
+    end)
+| bnd o1 o2 B => bnd o1 o2 (substitution_depth B depth i1 i2)
+| prd vec pn pure => prd (vec_map (fun n => if nat_eqb n i1 then i2 else n) vec) pn pure
 end.
 
 Fixpoint substitution (A : formula) (i1 i2 : ivar) : formula :=
@@ -119,14 +214,75 @@ match A with
     | false, false => A
     end
 | imp B C => imp (substitution B i1 i2) (substitution C i1 i2)
-| univ v B => 
-    (match nat_eqb v i1 with
-    | true => A
-    | false => univ v (substitution B i1 i2)
-    end)
+| univ B => univ (substitution B i1 i2)
 | bnd o1 o2 B => bnd o1 o2 (substitution B i1 i2)
-| prd pn _ => A
+| prd vec pn pure => prd (vec_map (fun n => if nat_eqb n i1 then i2 else n) vec) pn pure
 end.
+
+Lemma vec_map_ext {n : nat} :
+    forall (F G : nat -> nat),
+        F = G ->
+          forall (vec : nvec n),
+              vec_map F vec = vec_map G vec.
+Proof.
+intros F G FEQ vec.
+rewrite FEQ.
+reflexivity.
+Qed.
+
+Lemma vec_map_id {n : nat} :
+    forall (vec : nvec n),
+              vec_map (fun n => n) vec = vec.
+Proof.
+induction vec.
+reflexivity.
+unfold vec_map;
+fold @vec_map.
+rewrite IHvec.
+reflexivity.
+Qed.
+
+Lemma vec_map_app {n : nat} :
+    forall (F G : nat -> nat) (vec : nvec n),
+        vec_map F (vec_map G vec) = vec_map (fun n => (F (G n))) vec.
+Proof.
+intros F G.
+induction vec.
+reflexivity.
+unfold vec_map;
+fold @vec_map.
+rewrite IHvec.
+reflexivity.
+Qed.
+
+Lemma subst_depth_eq_refl : forall (A : formula) (n : nat) (i : ivar), substitution_depth A n i i = A.
+Proof.
+induction A;
+intros n' iv;
+unfold substitution_depth;
+fold substitution_depth;
+try rewrite IHA;
+try rewrite IHA1;
+try rewrite IHA2;
+try reflexivity.
+1 : case (nat_eqb i iv) eqn:EQ1;
+    case (nat_eqb i0 iv) eqn:EQ2;
+    try apply nat_eqb_eq in EQ1;
+    try apply nat_eqb_eq in EQ2;
+    subst;
+    reflexivity.
+1 : case (nat_ltb n' iv) eqn:EQ;
+    reflexivity.
+1 : assert ((fun n0 => if nat_eqb n0 iv then iv else n0) = (fun n => n)) as EQ.
+    { apply functional_extensionality.
+      intros x.
+      case (nat_eqb x iv) eqn:EQ.
+      apply nat_eqb_eq in EQ.
+      rewrite EQ.
+      all : reflexivity. }
+    rewrite (vec_map_ext _ _ EQ), vec_map_id.
+    reflexivity.
+Qed.
 
 Lemma subst_eq_refl : forall (A : formula) (i : ivar), substitution A i i = A.
 Proof.
@@ -138,20 +294,67 @@ try rewrite IHA;
 try rewrite IHA1;
 try rewrite IHA2;
 try reflexivity.
-all : case (nat_eqb i iv) eqn:EQ1;
-      try reflexivity.
-all : case (nat_eqb i0 iv) eqn:EQ2;
-      try apply nat_eqb_eq in EQ1;
-      try apply nat_eqb_eq in EQ2;
-      subst;
-      reflexivity.
+1 : case (nat_eqb i iv) eqn:EQ1;
+    case (nat_eqb i0 iv) eqn:EQ2;
+    try apply nat_eqb_eq in EQ1;
+    try apply nat_eqb_eq in EQ2;
+    subst;
+    reflexivity.
+1 : assert ((fun n0 => if nat_eqb n0 iv then iv else n0) = (fun n => n)) as EQ.
+    { apply functional_extensionality.
+      intros x.
+      case (nat_eqb x iv) eqn:EQ.
+      apply nat_eqb_eq in EQ.
+      rewrite EQ.
+      all : reflexivity. }
+    rewrite (vec_map_ext _ _ EQ), vec_map_id.
+    reflexivity.
+Qed.
+
+Lemma subst_forms_equiv_for_free_var_aux :
+    forall (phi : formula) (v1 v2 : ivar) (n : nat),
+        nat_ltb (form_depth phi + n) v1 = true ->
+            nat_ltb (form_depth phi + n) v2 = true ->
+                substitution_depth phi n v1 v2 = substitution phi v1 v2.
+Proof.
+induction phi;
+intros v1 v2 n' FV1 FV2;
+unfold substitution_depth;
+fold substitution_depth;
+unfold substitution;
+fold substitution;
+try reflexivity;
+unfold form_depth in *;
+fold form_depth in *;
+apply nat_ltb_lt in FV1, FV2.
+3 : rewrite IHphi.
+2 : assert (n' < v1 /\ n' < v2) as [LT1 LT2].
+2 : split; lia.
+2 : rewrite (nat_lt_ltb _ _ LT1), (nat_lt_ltb _ _ LT2), IHphi.  
+1 : rewrite IHphi1, IHphi2.
+all : try reflexivity;
+      apply nat_lt_ltb;
+      lia.
+Qed.
+
+Lemma subst_forms_equiv_for_free_var :
+    forall (phi : formula) (v1 v2 : ivar),
+        nat_ltb (form_depth phi) v1 = true ->
+            nat_ltb (form_depth phi) v2 = true ->
+                substitution_depth phi 0 v1 v2 = substitution phi v1 v2.
+Proof.
+intros phi v1 v2 LT1 LT2.
+apply subst_forms_equiv_for_free_var_aux;
+rewrite <- plus_n_O.
+apply LT1.
+apply LT2.
 Qed.
 
 Lemma nvec_case :
     forall (n : nat) (P : nvec n -> Type),
         (forall (pf : n = 0),
             P (eq_rect 0 nvec Null n (eq_sym pf))) ->
-        (forall (i m : nat) (vec : nvec i) (pf : n = S i), P (eq_rect (S i) nvec (New i m vec) n (eq_sym pf))) ->
+        (forall (m i : nat) (vec : nvec m) (pf : n = S m), P (eq_rect (S m) nvec (New i vec) n (eq_sym pf))) ->
             (forall (vec : nvec n), P vec).
 Proof.
 intros n P BC IND vec.
@@ -171,7 +374,7 @@ apply nvec_case.
   inversion pf.
 Qed.
 
-Lemma nvec_Sn_new : forall {n : nat} (vec : nvec (S n)), {subvec : nvec n & {m : nat & vec = New n m subvec}}.
+Lemma nvec_Sn_new : forall {n : nat} (vec : nvec (S n)), {subvec : nvec n & {m : nat & vec = New m subvec}}.
 Proof.
 intros n.
 apply nvec_case.
@@ -254,38 +457,35 @@ case (nvec_eqb a b) eqn:EQ.
 Qed.
 
 Lemma pred_case :
-    forall (n : nat) (vec : nvec n) (P : predicate vec -> Type),
-        (forall (i : nat) (pf : n = 0) (pfv : vec = (eq_rect 0 nvec Null n (eq_sym pf))),
-            P (eq_rect _ predicate (Nullary i pf) _ (eq_sym pfv))) ->
-        (forall (m : nat) (vec' : nvec m) (i : nat) (v : ivar) (prd : predicate vec') (pf : n = S m) (pfv : vec = eq_rect (S m) nvec (New m v vec') n (eq_sym pf)),
-            P (eq_rect _ predicate (Succary i v prd pf) _ (eq_sym pfv))) ->
+    forall (n : nat) (P : predicate n -> Type),
+        (forall (i : nat) (pf : n = 0),
+            P (eq_rect _ predicate (Nullary i) _ (eq_sym pf))) ->
+        (forall (m : nat) (i : nat) (prd : predicate m) (pf : n = S m),
+            P (eq_rect _ predicate (Succary i prd) _ (eq_sym pf))) ->
         (forall (i : nat), P (Var i)) ->
-            (forall (pn : predicate vec), P pn).
+            (forall (pn : predicate n), P pn).
 Proof.
-intros n vec P BC IND VARS pn.
-pose proof (Eqdep_dec.eq_rect_eq_dec nat_eq_dec nvec vec (eq_sym eq_refl)).
+intros n P BC IND VARS pn.
 induction pn.
-apply (BC _ pf eq_refl).
-apply (IND _ _ _ _ _ pf eq_refl).
+apply (BC _ eq_refl).
+apply (IND _ _ _ eq_refl).
 apply VARS.
 Qed.
 
 Lemma prd_eqb_sym :
-    forall {n1 n2 : nat} {vec1 : nvec n1} {vec2 : nvec n2} (pn1 : predicate vec1) (pn2 : predicate vec2),
+    forall {n1 n2 : nat} (pn1 : predicate n1) (pn2 : predicate n2),
         prd_eqb pn1 pn2 = prd_eqb pn2 pn1. 
 Proof.
-intros n1 n2 vec1 vec2 pn1.
-revert n2 vec2.
+intros n1 n2 pn1.
+revert n2.
 induction pn1;
-intros n2 vec2;
+intros n2;
 destruct pn2;
 unfold prd_eqb;
 fold @prd_eqb;
 subst;
 try rewrite !nat_eqb_refl;
-try rewrite nvec_eqb_refl;
 try rewrite nat_eqb_symm;
-try rewrite nvec_eqb_sym;
 try rewrite (nat_eqb_symm v v0);
 try rewrite (nat_eqb_symm i i0);
 try rewrite IHpn1;
@@ -293,55 +493,37 @@ reflexivity.
 Qed.
 
 Lemma prd_eqb_eq :
-    forall {n : nat} {vec : nvec n} (pn1 pn2 : predicate vec),
+    forall {n : nat} (pn1 pn2 : predicate n),
         prd_eqb pn1 pn2 = true ->
             pn1 = pn2.
 Proof.
-intros n vec.
-induction pn1.
-- intros pn2.
-  subst.
-  unfold eq_rect, eq_sym in *.
-  apply (pred_case 0 Null (fun (pn2 : predicate Null) => prd_eqb (Nullary i eq_refl) pn2 = true -> (Nullary i eq_refl) = pn2)).
-  + intros i1 pf pfv EQB.
-    rewrite pfv in EQB.
-    unfold eq_rect, eq_sym in EQB.
-    rewrite (UIP _ _ _ pf eq_refl) in EQB.
-    unfold prd_eqb in EQB.
-    rewrite nat_eqb_refl, nvec_eqb_refl in EQB.
+intros n.
+induction pn1;
+intros pn2.
+- apply (pred_case 0 (fun (pn2 : predicate 0) => prd_eqb (Nullary i) pn2 = true -> (Nullary i) = pn2)).
+  + intros i1 pf EQB.
+    rewrite pf in EQB.
+    unfold eq_rect, eq_sym, prd_eqb, nat_eqb in EQB.
     apply nat_eqb_eq in EQB.
     subst.
     pose proof (UIP_refl _ _ pf).
     subst.
-    unfold eq_rect, eq_sym in pfv.
-    pose proof (UIP_refl _ _ pfv).
-    subst.
     reflexivity.
-  + intros m vec i1 v pn1 pf pfv EQB.
+  + intros m i1 pn1 pf EQB.
     inversion pf.
   + intros i1 EQB.
     inversion EQB.
-- intros pn3.
-  subst.
-  unfold eq_rect, eq_sym in *.
-  apply (pred_case (S m) (New m v vec) (fun (pn2 : predicate (New m v vec)) => prd_eqb (Succary i v pn1 eq_refl) pn2 = true -> (Succary i v pn1 eq_refl) = pn2)).
-  + intros i1 pf pfv EQB.
+- apply (pred_case (S m) (fun (pn2 : predicate (S m)) => prd_eqb (Succary i pn1) pn2 = true -> (Succary i pn1) = pn2)).
+  + intros i1 pf EQB.
     inversion pf.
-  + intros m2 vec2 i2 v2 pn2 pf pfv EQB.
+  + intros m2 i2 pn3 pf EQB.
     inversion pf as [pf'].
     subst.
     pose proof (UIP_refl _ _ pf).
     subst.
-    unfold eq_rect, eq_sym in pfv.
-    inversion pfv as [[EQ1 EQ2]].
-    apply inj_pair2 in EQ2.
-    subst.
-    pose proof (UIP_refl _ _ pfv).
-    subst.
-    unfold eq_rect, eq_sym in *.
-    unfold prd_eqb in EQB;
+    unfold eq_rect, eq_sym, prd_eqb in EQB;
     fold @prd_eqb in EQB.
-    rewrite nat_eqb_refl, nvec_eqb_refl, nat_eqb_refl, andb_true_r in EQB.
+    rewrite nat_eqb_refl in EQB.
     apply and_bool_prop in EQB as [EQ1 EQ2].
     apply nat_eqb_eq in EQ1.
     specialize (IHpn1 _ EQ2) as EQ3.
@@ -349,77 +531,67 @@ induction pn1.
     reflexivity.
   + intros i1 EQB.
     unfold prd_eqb in EQB.
-    rewrite nat_eqb_refl, nvec_eqb_refl in EQB.
+    rewrite nat_eqb_refl in EQB.
     inversion EQB.
-- intros pn2.
-  apply (pred_case n vec (fun (pn2 : predicate vec) => prd_eqb (Var i) pn2 = true -> (Var i) = pn2)).
-  + intros i1 pf pfv EQB.
+- apply (pred_case n (fun (pn2 : predicate n) => prd_eqb (Var i) pn2 = true -> (Var i) = pn2)).
+  + intros i1 pf EQB.
     subst.
     inversion EQB.
-  + intros m vec2 i1 v pn1 pf pfv EQB.
+  + intros m i1 pn1 pf EQB.
     subst.
-    unfold prd_eqb in EQB.
-    rewrite nat_eqb_refl, nvec_eqb_refl in EQB.
+    unfold eq_rect, eq_sym, prd_eqb in EQB.
+    rewrite nat_eqb_refl in EQB.
     inversion EQB.
   + intros i2 EQB.
     unfold prd_eqb in EQB.
-    rewrite nat_eqb_refl, nvec_eqb_refl in EQB.
+    rewrite nat_eqb_refl in EQB.
     apply nat_eqb_eq in EQB.
     subst.
     reflexivity.
 Qed.
 
 Lemma prd_eqb_refl :
-    forall {n : nat} {vec : nvec n} (pn : predicate vec),
+    forall {n : nat} (pn : predicate n),
         prd_eqb pn pn = true.
 Proof.
-intros n vec pn.
+intros n pn.
 induction pn;
 unfold prd_eqb;
 fold @prd_eqb;
 repeat rewrite nat_eqb_refl;
-rewrite nvec_eqb_refl;
 try rewrite IHpn;
 try reflexivity.
 Qed.
 
 Lemma prd_eqb_type : 
-    forall {n1 n2 : nat} {vec1 : nvec n1} {vec2 : nvec n2} (pn1 : predicate vec1) (pn2 : predicate vec2),
-        prd_eqb pn1 pn2 = true -> nat_eqb n1 n2 = true /\ nvec_eqb vec1 vec2 = true.
+    forall {n1 n2 : nat} (pn1 : predicate n1) (pn2 : predicate n2),
+        prd_eqb pn1 pn2 = true -> nat_eqb n1 n2 = true .
 Proof.
-intros n1 n2 vec1 vec2 pn1 pn2 EQB.
+intros n1 n2 pn1 pn2 EQB.
 destruct pn1, pn2;
 subst;
 unfold prd_eqb, eq_rect, eq_sym in EQB;
 fold @prd_eqb in EQB.
-- split; reflexivity.
+- reflexivity.
 - inversion EQB.
-- case (nat_eqb 0 n2) eqn:EQ1;
-  case (nvec_eqb Null vec) eqn:EQ2;
+- case (nat_eqb 0 n) eqn:EQ1;
   inversion EQB.
 - inversion EQB.
-- unfold eq_rect, eq_sym.
-  case (nat_eqb (S m) (S m0)) eqn:EQ1.
-  case (nvec_eqb (New m v vec) (New m0 v0 vec0)) eqn:EQ2.
-  split; reflexivity.
+- case (nat_eqb (S m) (S m0)) eqn:EQ1.
+  reflexivity.
   inversion EQB.
+- case (nat_eqb (S m) n) eqn:EQ1;
   inversion EQB.
-- case (nat_eqb (S m) n2) eqn:EQ1;
-  case (nvec_eqb (New m v vec) vec0) eqn:EQ2;
+- case (nat_eqb n 0) eqn:EQ1;
   inversion EQB.
-- case (nat_eqb n1 0) eqn:EQ1;
-  case (nvec_eqb vec Null) eqn:EQ2;
+- case (nat_eqb n (S m)) eqn:EQ1;
   inversion EQB.
-- case (nat_eqb n1 (S m)) eqn:EQ1;
-  case (nvec_eqb vec (New m v vec0)) eqn:EQ2;
-  inversion EQB.
-- case (nat_eqb n1 n2) eqn:EQ1;
-  case (nvec_eqb vec vec0) eqn:EQ2;
-  inversion EQB.
-  split; reflexivity.
+- case (nat_eqb n n0) eqn:EQ1;
+  inversion EQB;
+  reflexivity.
 Qed.
 
-Definition prd_eq_dec {n : nat} {vec : nvec n} : forall (a b : predicate vec), {a = b} + {a <> b}.
+Definition prd_eq_dec {n : nat} : forall (a b : predicate n), {a = b} + {a <> b}.
 intros a b.
 case (prd_eqb a b) eqn:EQ.
 - left. apply prd_eqb_eq, EQ.
@@ -447,19 +619,18 @@ try apply nat_eqb_eq in EQ1 as [].
 - reflexivity.
 - rewrite (IHA1 _ EQ),(IHA2 _ EQ0).
   reflexivity.
-- rewrite (IHA _ EQ0).
+- rewrite (IHA _ EQ').
   reflexivity.
 - rewrite (IHA _ EQ0).
   reflexivity.
-- destruct (prd_eqb_type _ _ EQ') as [EQ1 EQ2].
-  apply nat_eqb_eq in EQ1.
+- apply and_bool_prop in EQ' as [EQ1 EQ2].
+  pose proof (prd_eqb_type _ _ EQ2) as EQ3.
+  apply nat_eqb_eq in EQ3.
   subst.
-  apply nvec_eqb_eq in EQ2.
+  apply nvec_eqb_eq in EQ1.
+  apply prd_eqb_eq in EQ2.
   subst.
-  apply prd_eqb_eq in EQ'.
-  subst.
-  pose proof (UIP  _ _ _ e e0).
-  subst.
+  rewrite (UIP  _ _ _ e e0).
   reflexivity.
 Qed.
 
@@ -474,6 +645,7 @@ try rewrite IHa;
 try rewrite IHa1;
 try rewrite IHa2;
 try reflexivity.
+rewrite nvec_eqb_refl.
 apply prd_eqb_refl.
 Qed.
 
@@ -488,16 +660,250 @@ case (form_eqb a b) eqn:EQ.
   inversion EQ.
 Qed.
 
-(*
-Fixpoint vec_map {n : nat} (F : nat -> nat) (vec : nvec n) : nvec n :=
-match n as n' return n' = n -> nvec n with
-| 0 => fun pf => (eq_rect _ _ Null _ pf)
-| S m => match vec with
-    | Null => fun pf => Null
-    | New _ v vec' => fun pf => New _ (F v) (vec_map F vec')
-    end
-end eq_refl.
-*)
+
+Fixpoint nvec_equiv {n1 n2 : nat} (vec1 : nvec n1) (vec2 : nvec n2) (diff : ivar) : bool :=
+match vec1, vec2 with
+| Null, Null => true
+| New v1 vec1', New v2 vec2' => (nat_eqb v1 v2 || nat_eqb (v1 + diff) v2) && nvec_equiv vec1' vec2' diff
+| _, _ => false
+end.
+
+Lemma nvec_equiv_0_eq {n : nat} :
+    forall (vec1 vec2 : nvec n),
+        nvec_equiv vec1 vec2 0 = true ->
+            vec1 = vec2.
+Proof.
+induction vec1.
+- apply (nvec_case _ (fun (vec2 : nvec 0) => nvec_equiv Null vec2 0 = true -> Null = vec2)).
+  + intros pf EQ.
+    rewrite (UIP_refl _ _ pf) in *.
+    reflexivity.
+  + intros m i vec pf EQ.
+    inversion pf.
+- apply (nvec_case _ (fun vec2 => nvec_equiv (New n vec1) vec2 0 = true -> (New n vec1) = vec2)).
+  + intros pf EQ'.
+    inversion pf.
+  + intros m' i vec2 pf EQ.
+    inversion pf as [pf'].
+    subst.
+    rewrite (UIP_refl _ _ pf) in *.
+    unfold eq_rect, eq_sym in *.
+    apply and_bool_prop in EQ as [EQ1 EQ2].
+    rewrite <- plus_n_O, orb_diag in EQ1.
+    apply nat_eqb_eq in EQ1.
+    subst.
+    rewrite (IHvec1 _ EQ2).
+    reflexivity.
+Qed.
+
+
+Lemma nvec_equiv_0_eqb {n1 n2 : nat} :
+    forall (vec1 : nvec n1) (vec2 : nvec n2),
+        nvec_equiv vec1 vec2 0 = nvec_eqb vec1 vec2.
+Proof.
+intros vec1.
+revert n2.
+induction vec1;
+induction vec2;
+unfold nvec_equiv;
+fold @nvec_equiv;
+unfold nvec_eqb;
+fold @nvec_eqb;
+try rewrite <- plus_n_O, orb_diag;
+try rewrite IHvec1;
+try reflexivity.
+Qed.
+
+Lemma nvec_vec_map_shift {n : nat} :
+    forall (vec : nvec n) (v1 v2 : ivar),
+        nvec_equiv vec (vec_map (fun m => if nat_eqb m v1 then m + v2 else m) vec) v2 = true.
+Proof.
+induction vec;
+intros v1 v2;
+unfold vec_map;
+fold @vec_map;
+unfold nvec_equiv;
+fold @nvec_equiv.
+reflexivity.
+rewrite IHvec.
+case (nat_eqb n v1) eqn:EQ;
+rewrite nat_eqb_refl;
+try rewrite orb_true_r;
+reflexivity.
+Qed.
+
+Lemma nvec_equiv_refl {n : nat} :
+    forall (vec : nvec n) (diff: ivar),
+        nvec_equiv vec vec diff = true.
+Proof.
+induction vec;
+intros diff;
+unfold nvec_equiv;
+fold @nvec_equiv;
+try rewrite IHvec;
+try rewrite nat_eqb_refl;
+reflexivity.
+Qed.
+
+Fixpoint form_equiv (A1 A2 : formula) (diff : ivar) : bool :=
+match A1, A2 with
+| fal, fal => true
+| equ v1 v2, equ v3 v4 => (nat_eqb v1 v3 || nat_eqb (v1 + diff) v3) && (nat_eqb v2 v4 || nat_eqb (v2 + diff) v4)
+| imp B1 C1, imp B2 C2 => form_equiv B1 B2 diff && form_equiv C1 C2 diff
+| univ B1, univ B2 => form_equiv B1 B2 diff
+| bnd lambda1 kappa1 B1, bnd lambda2 kappa2 B2 => nat_eqb lambda1 lambda2 && nat_eqb kappa1 kappa2 && form_equiv B1 B2 diff
+| prd vec1 pn1 _, prd vec2 pn2 _ => nvec_equiv vec1 vec2 diff && prd_eqb pn1 pn2
+| _, _ => false
+end.
+
+Lemma form_equiv_preserves_depth :
+    forall (A1 A2 : formula) (d : nat),
+        form_equiv A1 A2 d = true ->
+            form_depth A1 = form_depth A2.
+Proof.
+induction A1;
+destruct A2;
+intros d EQ;
+inversion EQ as [EQ'];
+unfold form_depth;
+fold form_depth;
+try apply and_bool_prop in EQ' as [EQ1 EQ2];
+try rewrite (IHA1 _ _ EQ');
+try rewrite (IHA1 _ _ EQ2);
+try rewrite (IHA1_1 _ _ EQ1);
+try rewrite (IHA1_2 _ _ EQ2);
+try reflexivity.
+Qed.
+
+Lemma form_equiv_preserves_ovars :
+    forall (A1 A2 : formula) (d : nat),
+        form_equiv A1 A2 d = true ->
+            vars_in A1 = vars_in A2.
+Proof.
+induction A1;
+destruct A2;
+intros d EQ;
+inversion EQ as [EQ'];
+unfold vars_in;
+fold vars_in;
+repeat apply and_bool_prop in EQ' as [EQ' ?EQ];
+try apply nat_eqb_eq in EQ';
+try apply nat_eqb_eq in EQ1;
+subst;
+try rewrite (IHA1 _ _ EQ');
+try rewrite (IHA1 _ _ EQ0);
+try rewrite (IHA1_1 _ _ EQ');
+try rewrite (IHA1_2 _ _ EQ0);
+try reflexivity.
+Qed.
+
+
+Lemma form_equiv_0_eq : 
+    forall (phi1 phi2 : formula),
+        form_equiv phi1 phi2 0 = form_eqb phi1 phi2.
+Proof.
+induction phi1;
+destruct phi2;
+unfold form_equiv;
+fold form_equiv;
+unfold form_eqb;
+fold form_eqb;
+try rewrite IHphi1;
+try rewrite IHphi1_1, IHphi1_2;
+try rewrite nat_eqb_refl;
+try rewrite nvec_equiv_0_eqb;
+try rewrite <- !plus_n_O, !orb_diag;
+reflexivity.
+Qed.
+
+Lemma form_equiv_diff_shift_subst :
+    forall (phi : formula) (v1 v2 : ivar),
+        form_equiv phi (shift_substitution phi v1 v2) v2 = true.
+Proof. 
+induction phi;
+intros v1 v2;
+unfold shift_substitution;
+fold shift_substitution;
+unfold form_equiv;
+fold form_equiv;
+try rewrite !nat_eqb_refl;
+try rewrite prd_eqb_refl;
+try rewrite IHphi;
+try rewrite IHphi1, IHphi2;
+try rewrite nvec_vec_map_shift;
+try reflexivity.
+case (nat_eqb i v1) eqn:EQ1;
+case (nat_eqb i0 v1) eqn:EQ2;
+try apply nat_eqb_eq in EQ1;
+try apply nat_eqb_eq in EQ2;
+subst;
+try rewrite !nat_eqb_refl;
+try rewrite !orb_true_l;
+try rewrite !orb_true_r;
+reflexivity.
+Qed.
+
+Lemma shift_subst_idem :
+    forall (phi : formula) (v1 v2 : ivar),
+        shift_substitution (shift_substitution phi v1 v2) v1 v2 = shift_substitution phi v1 v2.
+Proof.
+induction phi;
+intros v1 v2;
+unfold shift_substitution;
+fold shift_substitution;
+try rewrite IHphi;
+try rewrite IHphi1, IHphi2;
+try reflexivity.
+- case (nat_eqb i v1) eqn:EQ1;
+  case (nat_eqb i0 v1) eqn:EQ2;
+  try apply nat_eqb_eq in EQ1;
+  try apply nat_eqb_eq in EQ2;
+  subst;
+  unfold shift_substitution;
+  fold shift_substitution;
+  try rewrite EQ1;
+  try rewrite EQ2;
+  case (nat_eqb (v1 + v2) v1) eqn:EQ3;
+  try apply nat_eqb_eq in EQ3;
+  try rewrite !EQ3;
+  reflexivity.
+- rewrite vec_map_app.
+  rewrite <- (vec_map_ext (fun n0 => if nat_eqb n0 v1 then n0 + v2 else n0)).
+  reflexivity.
+  apply functional_extensionality.
+  intros m.
+  case (nat_eqb m v1) eqn:EQ.
+  + apply nat_eqb_eq in EQ;
+    subst.
+    destruct v2.
+    rewrite <- !plus_n_O, nat_eqb_refl.
+    reflexivity.
+    case (nat_eqb (v1 + S v2) v1) eqn:EQ.
+    apply nat_eqb_eq in EQ.
+    rewrite !EQ.
+    reflexivity.
+    reflexivity.
+  + rewrite EQ.
+    reflexivity.
+Qed.
+
+
+Lemma form_equiv_refl :
+    forall (phi : formula) (d : nat),
+        form_equiv phi phi d = true.
+Proof.
+induction phi;
+intros d;
+unfold form_equiv;
+fold form_equiv;
+try rewrite !nat_eqb_refl;
+try rewrite prd_eqb_refl;
+try rewrite !orb_true_l;
+try rewrite IHphi;
+try rewrite IHphi1, IHphi2;
+try rewrite nvec_equiv_refl;
+try reflexivity.
+Qed.
 
 (*
 Fixpoint sig_subst (a : formula) (sig : ovar -> ovar) : formula :=
