theories/Logic/inverse_ug_l.v
@@ -9,15 +9,30 @@ From Cyclic_PA.Logic Require Import proof_trees.
 From Cyclic_PA.Logic Require Import substitute.
 
 Require Import List.
+Require Import Lia.
 Import ListNotations.
 
-Definition ug_left_inv_formula (phi A : formula) (v : ivar) (b : bool) : formula := formula_sub phi (univ v A) A b.
+Definition ug_left_inv_formula (phi A : formula) (b : bool) : formula := formula_sub phi (univ A) A 0 b.
 
-Definition ug_left_inv_batch (gamma : list formula) (A : formula) (v : ivar) (S : subst_ind) : list formula := batch_sub gamma (univ v A) A S.
+Lemma ug_l_inv_form_depth_le :
+    forall (phi A : formula) (b : bool),
+        form_depth (formula_sub phi (univ A) A 0 b) <= form_depth phi.
+Proof.
+intros phi A b.
+unfold formula_sub.
+case form_equiv eqn:EQF.
+destruct b.
+rewrite (form_equiv_preserves_depth _ _ _ EQF).
+unfold form_depth;
+fold form_depth.
+all : lia.
+Qed.
+
+Definition ug_left_inv_batch (gamma : list formula) (A : formula) (d : nat) (S : subst_ind) : list formula := batch_sub gamma (univ A) A d S.
 
 Fixpoint ptree_ug_l_inv_fit
-  (P : ptree) (A : formula) (i : ivar) (S : subst_ind) : ptree :=
-let REC := (fun PT SI => (ptree_ug_l_inv_fit PT A i SI)) in
+  (P : ptree) (A : formula) (S : subst_ind) : ptree :=
+let REC := (fun PT SI => (ptree_ug_l_inv_fit PT A SI)) in
 match P, S with
 | bot, _ => P
 
@@ -25,17 +40,17 @@ match P, S with
 
 | equal v1 v2, _ => P
 
-| loop_head OC gamma delta alpha P_Target, _ => loop_head OC (ug_left_inv_batch gamma A i S) delta alpha (REC P_Target S)
+| loop_head OC gamma delta alpha P_Target, _ => loop_head OC (ug_left_inv_batch gamma A 0 S) delta alpha (REC P_Target S)
 
-| @con_l OC gamma delta phi alpha P', s :: S' => @con_l OC (ug_left_inv_batch gamma A i S') delta (ug_left_inv_formula phi A i s) alpha (REC P' (s :: s :: S'))
+| @sub_l OC gamma delta phi v1 v2 alpha P', s1 :: s2 :: S' => @sub_l OC (ug_left_inv_batch gamma A 0 S') delta (formula_sub (shift_substitution phi v1 v2) (univ A) A v2 s2) v1 v2 alpha (REC P' (s1 :: s2 :: S'))
+
+| @sub_r OC gamma delta phi v1 v2 alpha P', s :: S' => @sub_r OC (ug_left_inv_batch gamma A 0 S') delta phi v1 v2 alpha (REC P' (s :: S'))
+
+| @con_l OC gamma delta phi alpha P', s :: S' => @con_l OC (ug_left_inv_batch gamma A 0 S') delta (ug_left_inv_formula phi A s) alpha (REC P' (s :: s :: S'))
 
 | @con_r OC gamma delta phi alpha P', _ => @con_r OC (ptree_left (REC P' S)) delta phi alpha (REC P' S)
 
-| @sub_l OC gamma delta phi v1 v2 alpha P', s1 :: s2 :: S' => @sub_l OC (ug_left_inv_batch gamma A i S') delta (ug_left_inv_formula phi A i s2) v1 v2 alpha (REC P' (s1 :: s2 :: S'))
-
-| @sub_r OC gamma delta phi v1 v2 alpha P', s :: S' => @sub_r OC (ug_left_inv_batch gamma A i S') delta phi v1 v2 alpha (REC P' (s :: S'))
-
-| @refl OC gamma delta v alpha P', _ => @refl OC (ug_left_inv_batch gamma A i S) delta v alpha (ptree_ug_l_inv_fit P' A i (false :: S))
+| @refl OC gamma delta v alpha P', _ => @refl OC (ug_left_inv_batch gamma A 0 S) delta v alpha (ptree_ug_l_inv_fit P' A (false :: S))
 
 
 | @ex_l OC gamma delta n alpha P', _ => @ex_l OC (ptree_left (REC P' (unbury S n))) delta n alpha (REC P' (unbury S n))
@@ -43,56 +58,55 @@ match P, S with
 | @ex_r OC gamma delta n alpha P', _ => @ex_r OC (ptree_left (REC P' S)) delta n alpha (REC P' S)
 
 
-| @wkn_l OC gamma delta phi alpha P', s :: S' => @wkn_l OC (ug_left_inv_batch gamma A i S') delta (ug_left_inv_formula phi A i s) alpha (REC P' S')
+| @wkn_l OC gamma delta phi alpha P', s :: S' => @wkn_l OC (ug_left_inv_batch gamma A 0 S') delta (ug_left_inv_formula phi A s) alpha (REC P' S')
 
 | @wkn_r OC gamma delta phi alpha P', _ => @wkn_r OC (ptree_left (REC P' S)) delta phi alpha (REC P' S)
 
 | @rst OC gamma delta kappa alpha P', _ => @rst OC (ptree_left (REC P' S)) delta kappa alpha (REC P' S)
 
-| @ug_l OC gamma delta phi v alpha P', s :: S' => match nat_eqb v i && form_eqb phi A, s with
+| @ug_l OC gamma delta phi alpha P', s :: S' => match form_eqb phi A, s with
     | true, true => REC P' (false :: S')
-    | _, _ => let SI := (false :: S') in @ug_l OC (ug_left_inv_batch gamma A i S') delta phi v alpha (REC P' SI)
+    | _, _ => let SI := (false :: S') in @ug_l OC (ug_left_inv_batch gamma A 0 S') delta phi alpha (REC P' SI)
     end
 
-| @ug_r OC gamma delta phi v alpha P', _ => @ug_r OC (ptree_left (REC P' S)) delta phi v alpha (REC P' S)
+| @ug_r OC gamma delta phi alpha P', _ => @ug_r OC (ptree_left (REC P' S)) delta phi alpha (REC P' S)
 
-| @bnd_l OC gamma delta phi lambda kappa alpha P', s :: S' => @bnd_l OC (ug_left_inv_batch gamma A i S') delta phi lambda kappa alpha (REC P' (false :: S'))
+| @bnd_l OC gamma delta phi lambda kappa alpha P', s :: S' => @bnd_l OC (ug_left_inv_batch gamma A 0 S') delta phi lambda kappa alpha (REC P' (false :: S'))
 
 | @bnd_r OC gamma delta phi lambda kappa alpha P', _ => @bnd_r OC (ptree_left (REC P' S)) delta phi lambda kappa alpha (REC P' S)
 
-| @imp_l OC gamma delta phi psi alpha1 alpha2 P1 P2, s :: S' =>  @imp_l OC (ug_left_inv_batch gamma A i S') delta phi psi alpha1 alpha2 (REC P1 (false :: S')) (REC P2 S')
+| @imp_l OC gamma delta phi psi alpha1 alpha2 P1 P2, s :: S' =>  @imp_l OC (ug_left_inv_batch gamma A 0 S') delta phi psi alpha1 alpha2 (REC P1 (false :: S')) (REC P2 S')
 
-| @imp_r OC gamma delta phi psi alpha P', _ => @imp_r OC (ug_left_inv_batch gamma A i S) delta phi psi alpha (REC P' (false :: S))
+| @imp_r OC gamma delta phi psi alpha P', _ => @imp_r OC (ug_left_inv_batch gamma A 0 S) delta phi psi alpha (REC P' (false :: S))
 
-| @cut OC gamma delta phi alpha1 alpha2 P1 P2, _ => @cut OC (ug_left_inv_batch gamma A i S) delta phi alpha1 alpha2 (REC P1 S) (REC P2 (false :: S))
+| @cut OC gamma delta phi alpha1 alpha2 P1 P2, _ => @cut OC (ug_left_inv_batch gamma A 0 S) delta phi alpha1 alpha2 (REC P1 S) (REC P2 (false :: S))
 
 | _ , _ => P
 end.
 
-Definition ptree_ug_l_inv (P : ptree) (A : formula) (i : ivar) (S : subst_ind) : ptree :=
+Definition ptree_ug_l_inv (P : ptree) (A : formula) (S : subst_ind) : ptree :=
 match nat_eqb (length (ptree_left P)) (length S) with
-| true => ptree_ug_l_inv_fit P A i S
+| true => ptree_ug_l_inv_fit P A S
 | false => P
 end.
 
 Lemma ptree_ug_l_inv_fit_true :
-    forall {P : ptree} {A : formula} {v : ivar},
+    forall {P : ptree} {A : formula},
         forall {S : subst_ind},
             nat_eqb (length (ptree_left P)) (length S) = true ->
-                (ptree_ug_l_inv_fit P A v S) = (ptree_ug_l_inv P A v S).
-Proof. intros P A v S EQ. unfold ptree_ug_l_inv. rewrite EQ. reflexivity. Qed.
+                (ptree_ug_l_inv_fit P A S) = (ptree_ug_l_inv P A S).
+Proof. intros P A S EQ. unfold ptree_ug_l_inv. rewrite EQ. reflexivity. Qed.
 
 Lemma ptree_ug_l_inv_left :
-    forall (P : ptree) (A : formula) (v : ivar),
+    forall (P : ptree) (A : formula),
         struct_valid P ->
-            weak_formula A = false ->
-                forall (S : subst_ind),
-                    ptree_left (ptree_ug_l_inv P A v S) =
-                        (ug_left_inv_batch (ptree_left P) A v S).
+            forall (S : subst_ind),
+                ptree_left (ptree_ug_l_inv P A S) =
+                    (ug_left_inv_batch (ptree_left P) A 0 S).
 Proof.
-intros P A v.
+intros P A.
 induction P;
-try intros PSV WF S;
+try intros PSV S;
 unfold ptree_ug_l_inv;
 unfold ug_left_inv_batch, batch_sub;
 case nat_eqb eqn:EQ;
@@ -103,9 +117,8 @@ unfold ptree_left in EQ;
 fold ptree_left in EQ.
 
 1-3 : destruct PSV.
-4 : destruct PSV as [[[PSV [PG_app PD_app]] [PBot | [[[[PRec PG] PD] POC] PDeg]]] PWF].
-6-12 : destruct PSV as [[[[[PSV [PG_app PD_app]] PG] PD] POC] PDeg].
-13-14 : destruct PSV as [[[[[[PSV [PG_app PD_app]] PG] PD] POC] PDeg] PWF].
+4 : destruct PSV as [[PSV [PG_app PD_app]] [PBot | [[[[PRec PG] PD] POC] PDeg]]].
+6-14 : destruct PSV as [[[[[PSV [PG_app PD_app]] PG] PD] POC] PDeg].
 15 : destruct PSV as [[[[[[[PSV [PG_app PD_app]] PG] PD] KNING] KNIND] [KIN POC]] PDeg].
 16-17 : destruct PSV as [[[[[PSV [PG_app PD_app]] PG] PD] POC] PDeg].
 18 : destruct PSV as [[[[[[PSV [PG_app PD_app]] PG] PD] POC] POC_rel] PDeg].
@@ -120,9 +133,9 @@ all : subst;
       unfold batch_sub_fit;
       fold @batch_sub_fit.
 
-7,12,14,15,17,19 :  rewrite (batch_sub_fit_true EQ);
+9,12,14,15,17,19 :  rewrite (batch_sub_fit_true EQ);
                     rewrite (ptree_ug_l_inv_fit_true EQ);
-                    apply (IHP PSV WF).
+                    apply (IHP PSV).
 
 1-3 : destruct S;
       reflexivity.
@@ -130,124 +143,69 @@ all : subst;
 all : try rewrite (batch_sub_fit_true EQ);
       try reflexivity.
 
-- destruct S as [ | b S];
-  inversion EQ.
-  rewrite batch_sub_fit_true, ptree_ug_l_inv_fit_true.
-  reflexivity.
-  rewrite PG.
-  apply EQ.
-  apply EQ.
+1 : { destruct S as [ | b1 [ | b2 S]].
+      1,2 : inversion EQ.
+      unfold ptree_left.
+      unfold form_equiv, ug_left_inv_formula, ug_left_inv_batch.
+      rewrite batch_sub_fit_true.
+      2 : apply EQ.
+      admit. }
 
-- destruct S as [ | b1 [ | b2 S]].
-  1,2 : inversion EQ.
-  unfold ptree_left.
-  unfold formula_sub at 1.
-  unfold form_eqb, ug_left_inv_formula, ug_left_inv_batch.
-  rewrite batch_sub_fit_true.
-  2 : apply EQ.
-  unfold form_equiv at 1.
-  rewrite (form_sub_sub0_comm _ _ _ _ _ WF).
-  reflexivity.
+3 : { unfold ptree_left at 1.
+      fold (ptree_left (ptree_ug_l_inv_fit P A (unbury S n))).
+      rewrite ptree_ug_l_inv_fit_true, <- batch_bury_comm, (IHP PSV).
+      reflexivity.
+      rewrite bury_length, <- (@bury_unbury _ S n), bury_length in EQ.
+      apply EQ. }
 
-- destruct S as [ | b S].
-  inversion EQ.
-  rewrite batch_sub_fit_true.
-  reflexivity.
-  apply EQ.
+all : destruct S as [ | b S];
+      inversion EQ.
 
-- unfold ptree_left at 1.
-  fold (ptree_left (ptree_ug_l_inv_fit P A v (unbury S n))).
-  rewrite ptree_ug_l_inv_fit_true, <- batch_bury_comm, (IHP PSV WF).
-  reflexivity.
-  rewrite bury_length, <- (@bury_unbury _ S n), bury_length in EQ.
-  apply EQ.
+4 : unfold formula_sub, form_equiv;
+    fold form_equiv;
+    try rewrite form_equiv_0_eq;
+    case (form_eqb phi A) eqn:EQF.
+4 : destruct b.
 
-- destruct S as [ | b S].
-  inversion EQ.
-  unfold ptree_left at 1 2.
-  fold (ptree_left P).
-  unfold batch_sub, batch_sub_fit;
-  fold batch_sub_fit.
-  rewrite batch_sub_fit_true, EQ.
-  reflexivity.
-  apply EQ.
+all : try unfold ptree_left at 1 2;
+      try fold (ptree_left P);
+      try fold (ptree_left P2);
+      unfold batch_sub, batch_sub_fit;
+      fold batch_sub_fit;
+      try rewrite batch_sub_fit_true;
+      try rewrite EQ;
+      try apply EQ;
+      try reflexivity.
 
-- destruct S as [ | b S].
-  inversion EQ.
-  unfold formula_sub, form_eqb;
-  fold form_eqb.
-  case (nat_eqb v0 v && form_eqb phi A) eqn:EQ'.
-  case b.
-  + apply and_bool_prop in EQ' as [EQ1 EQ2].
-    apply form_eqb_eq in EQ2.
-    subst.
-    rewrite ptree_ug_l_inv_fit_true, (IHP PSV WF), PG.
+1 : rewrite ptree_ug_l_inv_fit_true, (IHP PSV), PG.
     unfold ug_left_inv_batch, batch_sub, batch_sub_fit at 1;
     fold batch_sub_fit.
     unfold length in *;
     fold (@length formula) (@length bool) in *.
-    rewrite EQ, formula_sub_false.
-    apply nat_eqb_eq in EQ1.
+    rewrite EQ, formula_sub_false, H0.
+    apply form_eqb_eq in EQF.
     subst.
-    rewrite form_equiv_refl.
     reflexivity.
     rewrite PG.
     apply EQ.
-  + unfold ptree_left.
-    rewrite batch_sub_fit_true.
-    apply and_bool_prop in EQ' as [EQ1 EQ2].
-    apply nat_eqb_eq in EQ1.
-    apply form_eqb_eq in EQ2.
-    subst.
-    rewrite form_equiv_refl.
-    reflexivity.
-    apply EQ.
-  + unfold ptree_left.
-    rewrite batch_sub_fit_true.
-    unfold form_equiv;
-    fold form_equiv.
-    case (nat_eqb v0 v) eqn:EQN;
-    try apply nat_eqb_eq in EQN;
-    subst;
-    rewrite (not_weak_equiv_eqb _ _ WF), EQ';
-    reflexivity.
-    apply EQ.
-
-- destruct S as [ | b S].
-  inversion EQ.
-  unfold ptree_left at 1, formula_sub, form_eqb.
-  rewrite batch_sub_fit_true.
-  reflexivity.
-  apply EQ.
-
-- destruct S as [ | b S].
-  inversion EQ.
-  unfold ptree_left at 1 2;
-  fold (ptree_left P2).
-  unfold batch_sub, batch_sub_fit;
-  fold batch_sub_fit.
-  rewrite batch_sub_fit_true, EQ.
-  reflexivity.
-  apply EQ.
-Qed.
+Admitted.
 
 Lemma ptree_ug_l_inv_right :
-    forall (P : ptree) (A : formula) (v : ivar),
+    forall (P : ptree) (A : formula),
         struct_valid P ->
             forall (S : subst_ind),
-                ptree_right (ptree_ug_l_inv P A v S) =
+                ptree_right (ptree_ug_l_inv P A S) =
                    (ptree_right P).
 Proof.
-intros P A v.
+intros P A.
 induction P;
 try intros PSV S;
 unfold ptree_ug_l_inv;
 unfold ug_left_inv_batch, batch_sub.
 
 1-3 : destruct PSV.
-4 : destruct PSV as [[[PSV [PG_app PD_app]] [PBot | [[[[PRec PG] PD] POC] PDeg]]] PWF].
-6-12 : destruct PSV as [[[[[PSV [PG_app PD_app]] PG] PD] POC] PDeg].
-13-14 : destruct PSV as [[[[[[PSV [PG_app PD_app]] PG] PD] POC] PDeg] PWF].
+4 : destruct PSV as [[PSV [PG_app PD_app]] [PBot | [[[[PRec PG] PD] POC] PDeg]]].
+6-14 : destruct PSV as [[[[[PSV [PG_app PD_app]] PG] PD] POC] PDeg].
 15 : destruct PSV as [[[[[[[PSV [PG_app PD_app]] PG] PD] KNING] KNIND] [KIN POC]] PDeg].
 16-17 : destruct PSV as [[[[[PSV [PG_app PD_app]] PG] PD] POC] PDeg].
 18 : destruct PSV as [[[[[[PSV [PG_app PD_app]] PG] PD] POC] POC_rel] PDeg].
@@ -264,42 +222,38 @@ all : subst;
       unfold ptree_left in EQ;
       fold ptree_left in EQ.
 
-1,3,4,6,7 : destruct S as [ | b S];
-        inversion EQ;
-        reflexivity.
+1 : destruct S as [ | b1 [ | b2 S]];
+    reflexivity.
 
-- destruct S as [ | b1 [ | b2 S]];
-  reflexivity.
+all : destruct S as [ | b S];
+      inversion EQ;
+      try case (form_eqb phi A) eqn:EQF;
+      case b;
+      try reflexivity.
 
-- destruct S as [ | b S].
-  inversion EQ.
-  case (nat_eqb v0 v && form_eqb phi A).
-  case b.
-  2,3 : reflexivity.
-  unfold ptree_right at 2.
-  rewrite ptree_ug_l_inv_fit_true.
-  apply (IHP PSV).
-  rewrite PG.
-  apply EQ.
+1 : unfold ptree_right at 2.
+    rewrite ptree_ug_l_inv_fit_true.
+    apply (IHP PSV).
+    rewrite PG.
+    apply EQ.
 Qed.
 
 Lemma ptree_ug_l_inv_constraint :
-    forall (P : ptree) (A : formula) (v : ivar),
+    forall (P : ptree) (A : formula),
         struct_valid P ->
             forall (S : subst_ind),
-                ptree_constraint (ptree_ug_l_inv P A v S) =
+                ptree_constraint (ptree_ug_l_inv P A S) =
                    (ptree_constraint P).
 Proof.
-intros P A v.
+intros P A.
 induction P;
 try intros PSV S;
 unfold ptree_ug_l_inv;
 unfold ug_left_inv_batch, batch_sub.
 
 1-3 : destruct PSV.
-4 : destruct PSV as [[[PSV [PG_app PD_app]] [PBot | [[[[PRec PG] PD] POC] PDeg]]] PWF].
-6-12 : destruct PSV as [[[[[PSV [PG_app PD_app]] PG] PD] POC] PDeg].
-13-14 : destruct PSV as [[[[[[PSV [PG_app PD_app]] PG] PD] POC] PDeg] PWF].
+4 : destruct PSV as [[PSV [PG_app PD_app]] [PBot | [[[[PRec PG] PD] POC] PDeg]]].
+6-14 : destruct PSV as [[[[[PSV [PG_app PD_app]] PG] PD] POC] PDeg].
 15 : destruct PSV as [[[[[[[PSV [PG_app PD_app]] PG] PD] KNING] KNIND] [KIN POC]] PDeg].
 16-17 : destruct PSV as [[[[[PSV [PG_app PD_app]] PG] PD] POC] PDeg].
 18 : destruct PSV as [[[[[[PSV [PG_app PD_app]] PG] PD] POC] POC_rel] PDeg].
@@ -316,42 +270,39 @@ all : subst;
       unfold ptree_left in EQ;
       fold ptree_left in EQ.
 
-1,3,4,6,7 : destruct S as [ | b S];
-            inversion EQ;
-            reflexivity.
 
-- destruct S as [ | b1 [ | b2 S]];
-  reflexivity.
+1 : destruct S as [ | b1 [ | b2 S]];
+    reflexivity.
+  
+all : destruct S as [ | b S];
+      inversion EQ;
+      try case (form_eqb phi A) eqn:EQF;
+      case b;
+      try reflexivity.
 
-- destruct S as [ | b S].
-  inversion EQ.
-  case (nat_eqb v0 v && form_eqb phi A).
-  case b.
-  2,3 : reflexivity.
-  unfold ptree_constraint at 2.
-  rewrite ptree_ug_l_inv_fit_true.
-  apply (IHP PSV).
-  rewrite PG.
-  apply EQ.
+1 : unfold ptree_constraint at 2.
+    rewrite ptree_ug_l_inv_fit_true.
+    apply (IHP PSV).
+    rewrite PG.
+    apply EQ.
 Qed.
 
 Lemma ptree_ug_l_inv_deg :
-    forall (P : ptree) (A : formula) (v : ivar),
+    forall (P : ptree) (A : formula),
         struct_valid P ->
             forall (S : subst_ind),
-                ptree_deg (ptree_ug_l_inv P A v S) =
+                ptree_deg (ptree_ug_l_inv P A S) =
                    (ptree_deg P).
 Proof.
-intros P A v.
+intros P A.
 induction P;
 try intros PSV S;
 unfold ptree_ug_l_inv;
 unfold ug_left_inv_batch, batch_sub.
 
 1-3 : destruct PSV.
-4 : destruct PSV as [[[PSV [PG_app PD_app]] [PBot | [[[[PRec PG] PD] POC] PDeg]]] PWF].
-6-12 : destruct PSV as [[[[[PSV [PG_app PD_app]] PG] PD] POC] PDeg].
-13-14 : destruct PSV as [[[[[[PSV [PG_app PD_app]] PG] PD] POC] PDeg] PWF].
+4 : destruct PSV as [[PSV [PG_app PD_app]] [PBot | [[[[PRec PG] PD] POC] PDeg]]].
+6-14 : destruct PSV as [[[[[PSV [PG_app PD_app]] PG] PD] POC] PDeg].
 15 : destruct PSV as [[[[[[[PSV [PG_app PD_app]] PG] PD] KNING] KNIND] [KIN POC]] PDeg].
 16-17 : destruct PSV as [[[[[PSV [PG_app PD_app]] PG] PD] POC] PDeg].
 18 : destruct PSV as [[[[[[PSV [PG_app PD_app]] PG] PD] POC] POC_rel] PDeg].
@@ -368,50 +319,43 @@ all : subst;
       unfold ptree_left in EQ;
       fold ptree_left in EQ.
 
-1,3,4,6,7 : destruct S as [ | b S];
-            inversion EQ;
-            reflexivity.
 
-- destruct S as [ | b1 [ | b2 S]];
-  reflexivity.
+1 : destruct S as [ | b1 [ | b2 S]];
+    reflexivity.
+  
+all : destruct S as [ | b S];
+      inversion EQ;
+      try case (form_eqb phi A) eqn:EQF;
+      case b;
+      try reflexivity.
 
-- destruct S as [ | b S].
-  inversion EQ.
-  case (nat_eqb v0 v && form_eqb phi A).
-  case b.
-  2,3 : reflexivity.
-  unfold ptree_deg at 2.
-  rewrite ptree_ug_l_inv_fit_true.
-  apply (IHP PSV).
-  rewrite PG.
-  apply EQ.
+1 : unfold ptree_deg at 2.
+    rewrite ptree_ug_l_inv_fit_true.
+    apply (IHP PSV).
+    rewrite PG.
+    apply EQ.
 Qed.
 
 Lemma ug_l_formula_inv_vars :
-    forall (phi : formula) (A : formula) (v : ivar) (b : bool),
-        weak_formula A = false ->
-            vars_in (ug_left_inv_formula phi A v b) =
-                vars_in phi.
+    forall (phi : formula) (A : formula) (b : bool),
+        vars_in (ug_left_inv_formula phi A b) =
+            vars_in phi.
 Proof.
-intros phi A v b WF.
+intros phi A b.
 unfold ug_left_inv_formula, formula_sub.
 case form_equiv eqn:EQF.
 destruct b.
-rewrite not_weak_equiv_eqb in EQF.
-apply form_eqb_eq in EQF.
-subst.
-all : try reflexivity.
-apply WF.
+rewrite (form_equiv_preserves_ovars _ _ _ EQF).
+all : reflexivity.
 Qed.
 
 Lemma ptree_ug_l_inv_vars :
-    forall (gamma : list formula) (A : formula) (v : ivar) (S : subst_ind),
-        weak_formula A = false ->
-            flat_map vars_in (ug_left_inv_batch gamma A v S) =
-                flat_map vars_in gamma.
+    forall (gamma : list formula) (A : formula) (S : subst_ind),
+        flat_map vars_in (ug_left_inv_batch gamma A 0 S) =
+            flat_map vars_in gamma.
 Proof.
 induction gamma;
-intros A v S WF;
+intros A S;
 unfold ug_left_inv_batch, batch_sub, batch_sub_fit;
 fold batch_sub_fit;
 destruct S;
@@ -422,19 +366,19 @@ case nat_eqb eqn:EQN.
 unfold flat_map;
 fold (flat_map vars_in).
 rewrite (batch_sub_fit_true EQN).
-fold (ug_left_inv_batch gamma A v S).
-rewrite (IHgamma _ _ _ WF).
-fold (ug_left_inv_formula a A v b).
-rewrite (ug_l_formula_inv_vars _ _ _ _ WF).
+fold (ug_left_inv_batch gamma A 0 S).
+rewrite IHgamma.
+fold (ug_left_inv_formula a A b).
+rewrite ug_l_formula_inv_vars.
 reflexivity.
 reflexivity.
 Qed.
 
 Lemma ptree_ug_l_inv_bot :
-    forall (phi : formula) (v : ivar) (S : subst_ind),
-        ptree_ug_l_inv bot phi v S = bot.
+    forall (phi : formula) (S : subst_ind),
+        ptree_ug_l_inv bot phi S = bot.
 Proof.
-intros phi v S.
+intros phi S.
 unfold ptree_ug_l_inv, ptree_ug_l_inv_fit.
 case (nat_eqb);
 reflexivity.
@@ -520,15 +464,14 @@ Qed.
 *)
 
 Lemma ptree_ug_l_inv_struct :
-    forall (P : ptree) (A : formula) (v : ivar),
+    forall (P : ptree) (A : formula),
         struct_valid P ->
-            weak_formula A = false ->
-                forall (S : subst_ind),
-                    struct_valid (ptree_ug_l_inv P A v S).
+            forall (S : subst_ind),
+                struct_valid (ptree_ug_l_inv P A S).
 Proof.
 intros P.
 induction P;
-try intros AF vf PSV WF S;
+try intros AF PSV S;
 unfold ptree_ug_l_inv;
 unfold ug_left_inv_batch, batch_sub;
 case nat_eqb eqn:EQ;
@@ -548,18 +491,17 @@ fold ptree_ug_l_inv_fit.
 9 : destruct S as [ | b S];
     try apply PSV.
 
-5 : destruct S as [ | b S];
+4 : destruct S as [ | b S];
     try apply PSV.
 
-4 : destruct S as [ | b1 [ | b2 S]];
+3 : destruct S as [ | b S];
     try apply PSV.
 
-2 : destruct S as [ | b S];
+2 : destruct S as [ | b1 [ | b2 S]];
     try apply PSV.
 
-1 : destruct PSV as [[[PSV [PG_app PD_app]] [PBot | [[[[PRec PG] PD] POC] PDeg]]] PWF].
-3-9 : destruct PSV as [[[[[PSV [PG_app PD_app]] PG] PD] POC] PDeg].
-10-11 : destruct PSV as [[[[[[PSV [PG_app PD_app]] PG] PD] POC] PDeg] PWF].
+1 : destruct PSV as [[PSV [PG_app PD_app]] [PBot | [[[[PRec PG] PD] POC] PDeg]]].
+3-11 : destruct PSV as [[[[[PSV [PG_app PD_app]] PG] PD] POC] PDeg].
 12 : destruct PSV as [[[[[[[PSV [PG_app PD_app]] PG] PD] KNING] KNIND] [KIN POC]] PDeg].
 13-14 : destruct PSV as [[[[[PSV [PG_app PD_app]] PG] PD] POC] PDeg].
 15 : destruct PSV as [[[[[[PSV [PG_app PD_app]] PG] PD] POC] POC_rel] PDeg].
@@ -570,22 +512,21 @@ fold ptree_ug_l_inv_fit.
 
 all : subst.
 
-13 :  case (nat_eqb v vf && form_eqb phi AF) eqn:EQfn;
+13 :  case (form_eqb phi AF) eqn:EQfn;
       case b.
 
 2 : { rewrite ptree_ug_l_inv_fit_true.
       2 : apply EQ.
-      enough (struct_valid (loop_head (ptree_constraint P) (ug_left_inv_batch (ptree_left P) AF vf S) (ptree_right P) (ptree_deg P) (ptree_ug_l_inv P AF vf S))) as PSV'.
+      enough (struct_valid (loop_head (ptree_constraint P) (ug_left_inv_batch (ptree_left P) AF 0 S) (ptree_right P) (ptree_deg P) (ptree_ug_l_inv P AF S))) as PSV'.
       destruct P;
       try apply PSV';
       contradiction (PRec eq_refl).
       repeat split.
-      - apply (IHP _ _ PSV WF).
+      - apply (IHP _ PSV).
       - rewrite ptree_ug_l_inv_vars.
         apply PG_app.
-        apply WF.
       - apply PD_app.
-      - destruct (ptree_eq_dec (ptree_ug_l_inv P AF vf S) bot) as [EQ' | NE].
+      - destruct (ptree_eq_dec (ptree_ug_l_inv P AF S) bot) as [EQ' | NE].
         apply (inl EQ').
         right.
         repeat split;
@@ -614,34 +555,13 @@ all : subst.
         try apply (IHP _ _ PSV);
         try apply (IHP1 _ _ P1SV);
         try apply (IHP2 _ _ P2SV);
-        try reflexivity.
-      - intros phi [INL | INR].
-        + unfold ug_left_inv_batch in INL.
-          rewrite batch_sub_is_map_combine in INL.
-          apply in_map_iff in INL as [[psi b] [EQF IN]].
-          apply in_combine_l in IN.
-          rewrite <- EQF.
-          unfold fst, snd.
-          refine (not_weak_sub_not_weak _ _ _ (PWF _ (or_introl IN)) WF _).
-          apply nat_eqb_eq, EQ.
-        + apply (PWF _ (or_intror INR)). }
+        try reflexivity. }
 
 1 : { repeat split.
       rewrite ptree_ug_l_inv_vars.
       apply PG_app.
-      apply WF.
       apply PD_app.
-      apply (inl eq_refl).
-      intros phi [INL | INR].
-      - unfold ug_left_inv_batch in INL.
-        rewrite batch_sub_is_map_combine in INL.
-        apply in_map_iff in INL as [[psi b] [EQF IN]].
-        apply in_combine_l in IN.
-        rewrite <- EQF.
-        unfold fst, snd.
-        refine (not_weak_sub_not_weak _ _ _ (PWF _ (or_introl IN)) WF _).
-        apply nat_eqb_eq, EQ.        
-      - apply (PWF _ (or_intror INR)). }
+      apply (inl eq_refl). }
 
 all : repeat rewrite ptree_ug_l_inv_fit_true;
       try rewrite PG;
@@ -666,9 +586,9 @@ all : repeat rewrite ptree_ug_l_inv_fit_true;
       try rewrite batch_sub_false_head;
       try rewrite ptree_ug_l_inv_right;
       try assumption;
-      try apply (IHP _ _ PSV WF);
-      try apply (IHP1 _ _ P1SV WF);
-      try apply (IHP2 _ _ P2SV WF);
+      try apply (IHP _ PSV);
+      try apply (IHP1 _ P1SV);
+      try apply (IHP2 _ P2SV);
       try reflexivity.
 
 all : try rewrite <- batch_sub_fit_true;
@@ -678,8 +598,16 @@ all : try rewrite <- batch_sub_fit_true;
       try reflexivity;
       try apply EQ.
 
-1 : rewrite <- (form_sub_sub0_comm _ _ _ _ _ WF).
-    reflexivity.
+- unfold formula_sub, form_equiv;
+  fold form_equiv.
+  case (form_equiv phi (univ AF) 0) eqn:EQF.
+  destruct b2.
+  rewrite form_equiv_0_eq in EQF.
+  apply form_eqb_eq in EQF.
+  subst.
+  rewrite form_equiv_diff_shift_subst.
 
-1 : apply (not_weak_sub_not_weak _ _ _ PWF WF).
+all : pose proof (ug_l_inv_form_depth_le phi AF b2) as LE;
+      unfold ug_left_inv_formula;
+      lia.
 Qed.
