theories/Logic/substitute.v
@@ -4,6 +4,8 @@ From Cyclic_PA.Logic Require Import definitions.
 From Cyclic_PA.Logic Require Import fol.
 
 Require Import List.
+Require Import Nat.
+Require Import Lia.
 Require Import Bool.
 Import ListNotations.
 
@@ -21,521 +23,381 @@ Definition non_target (gamma : list formula) : subst_ind := repeat false (length
 Definition target (gamma : list formula) : subst_ind := repeat true (length gamma).
 
 (*
-Definition formula_sub (phi A1 A2 : formula) (b : bool) : formula :=
-match form_eqb phi A1, b with
-| true, true => A2
-| _, _ => phi
+Fixpoint form_equiv (A1 A2 : formula) (depth : nat) : bool :=
+match A1, A2 with
+| fal, fal => true
+| equ v1 v2, equ v3 v4 => (nat_eqb v1 v3 || (nat_leb depth v1 && nat_leb depth v3)) && (nat_eqb v2 v4 || (nat_leb depth v2 && nat_leb depth v4))
+| imp B1 C1, imp B2 C2 => form_equiv B1 B2 depth && form_equiv C1 C2 depth
+| univ B1, univ B2 => form_equiv B1 B2 (S depth)
+| bnd lambda1 kappa1 B1, bnd lambda2 kappa2 B2 => nat_eqb lambda1 lambda2 && nat_eqb kappa1 kappa2 && form_equiv B1 B2 depth
+| prd vec1 pn1 _, prd vec2 pn2 _ => prd_eqb pn1 pn2
+| _, _ => false
 end.
 *)
 
-Fixpoint form_equiv (A1 A2 : formula) : bool :=
+(*
+Fixpoint form_equiv (A1 A2 : formula) (depth : nat) : bool :=
 match A1, A2 with
 | fal, fal => true
-| equ v1 v2, equ v3 v4 => (nat_eqb v3 0 || nat_eqb v1 v3) && (nat_eqb v4 0 || nat_eqb v2 v4)
-| imp B1 C1, imp B2 C2 => form_equiv B1 B2 && form_equiv C1 C2
-| univ v1 B1, univ v2 B2 => nat_eqb v1 v2 && form_equiv B1 B2
-| bnd o1 o2 B1, bnd o3 o4 B2 => nat_eqb o1 o3 && nat_eqb o2 o4 && form_equiv B1 B2
-| prd pn1 _, prd pn2 _ => prd_eqb pn1 pn2
+| equ v1 v2, equ v3 v4 =>
+    if nat_eqb v1 v2
+    then nat_eqb v3 v4
+    else (nat_eqb v1 v3 ||
+            (nat_leb depth v1 && nat_leb depth v3)) &&
+          (nat_eqb v2 v4 ||
+              (nat_leb depth v2 && nat_leb depth v4))
+| imp B1 C1, imp B2 C2 => form_equiv B1 B2 depth && form_equiv C1 C2 depth
+| univ B1, univ B2 => form_equiv B1 B2 (S depth)
+| bnd lambda1 kappa1 B1, bnd lambda2 kappa2 B2 => nat_eqb lambda1 lambda2 && nat_eqb kappa1 kappa2 && form_equiv B1 B2 depth
+| prd vec1 pn1 _, prd vec2 pn2 _ => prd_eqb pn1 pn2
 | _, _ => false
 end.
+*)
 
-Fixpoint weak_formula (A : formula) : bool :=
-match A with
-| fal => false
-| equ v1 v2 => nat_eqb v1 0 || nat_eqb v2 0
-| imp B C => weak_formula B || weak_formula C
-| univ v B => (* (negb (nat_eqb v 0)) && *) weak_formula B
-| bnd o1 o2 B => weak_formula B
-| prd pn pure => false
-end.
-
-Fixpoint binds0 (A : formula) : bool :=
-match A with
-| fal => false
-| equ v1 v2 => false
-| imp B C => binds0 B || binds0 C
-| univ v B => (nat_eqb v 0 && weak_formula B) || binds0 B
-| bnd o1 o2 B => binds0 B
-| prd pn pure => false
-end.
-
-Definition formula_sub (phi A1 A2 : formula) (b : bool) : formula :=
-match form_equiv phi A1, b with
-| true, true => A2
-| _, _ => phi
-end.
-
-Lemma form_equiv_refl :
-    forall (phi : formula),
-        form_equiv phi phi = true.
+(*
+Lemma form_equiv_shift_subst_aux :
+    forall (phi : formula) (v1 v2 : ivar) (d : nat),
+        d <= v1 ->
+        form_equiv phi (shift_substitution phi v1 v2) d = true.
 Proof.
 induction phi;
+intros v1 v2 d LT;
+unfold shift_substitution;
+fold shift_substitution;
 unfold form_equiv;
 fold form_equiv;
 try rewrite !nat_eqb_refl;
-try rewrite IHphi;
-try rewrite IHphi1, IHphi2;
-try rewrite !orb_true_r;
 try rewrite prd_eqb_refl;
-reflexivity.
+try rewrite IHphi;
+try rewrite IHphi1;
+try rewrite IHphi2;
+try reflexivity;
+unfold form_depth in *;
+fold form_depth in *;
+try lia.
+case (nat_eqb i v1) eqn:EQ1;
+case (nat_eqb i0 v1) eqn:EQ2;
+try apply nat_eqb_eq in EQ1;
+try apply nat_eqb_eq in EQ2;
+subst;
+try rewrite !nat_eqb_refl;
+try rewrite nat_eqb_symm in EQ2;
+try rewrite EQ2;
+try rewrite EQ1;
+try rewrite nat_eqb_symm in EQ1;
+try rewrite EQ1;
+assert (d <= v1 + v2) as LT';
+try lia;
+try rewrite (Compare_dec.leb_correct _ _ LT);
+try rewrite (Compare_dec.leb_correct _ _ LT');
+try rewrite !nat_eqb_refl;
+try rewrite !orb_true_l;
+try rewrite !orb_true_r;
+unfold "&&";
+try reflexivity.
+case (nat_eqb i i0); reflexivity.
 Qed.
+*)
 
-Lemma form_equiv_sub0 :
-    forall (phi : formula) (v : ivar),
-        form_equiv (substitution phi 0 v) phi = true.
+(*
+Lemma form_equiv_shift_subst :
+    forall (phi : formula) (v1 v2 : ivar),
+        form_equiv phi (shift_substitution phi v1 v2) 0 = true.
+Proof. intros phi v1 v2. apply form_equiv_shift_subst_aux. apply le_0_n. Qed.
+*)
+
+(*
+Lemma free_sub_means_equiv :
+    forall (phi : formula) (v1 v2 : ivar) (d : nat),
+        (form_depth phi) + d < v1 ->
+            (form_depth phi) + d < v2 ->
+                form_equiv (substitution phi v1 v2) phi d = true.
 Proof.
 induction phi;
-intros v;
+intros v1 v2 d LT1 LT2;
 unfold substitution;
 fold substitution;
+unfold form_depth;
+fold form_depth;
 unfold form_equiv;
 fold form_equiv;
-try case (nat_eqb i 0) eqn:EQ1;
-try case (nat_eqb i0 0) eqn:EQ2;
+try rewrite !nat_eqb_refl;
+try rewrite prd_eqb_refl;
+try rewrite IHphi;
+try rewrite IHphi1;
+try rewrite IHphi2;
+try reflexivity;
+unfold form_depth in *;
+fold form_depth in *;
+try lia.
+case (nat_eqb i v1) eqn:EQ1;
+case (nat_eqb i0 v1) eqn:EQ2;
 try apply nat_eqb_eq in EQ1;
 try apply nat_eqb_eq in EQ2;
 subst;
 unfold form_equiv;
 fold form_equiv;
 try rewrite !nat_eqb_refl;
-try rewrite IHphi;
-try rewrite IHphi1, IHphi2;
+try rewrite plus_O_n in *;
+try rewrite (nat_lt_ltb _ _ LT1);
+try rewrite (nat_lt_ltb _ _ LT2);
+try rewrite !orb_true_l;
 try rewrite !orb_true_r;
-try rewrite prd_eqb_refl;
-try rewrite form_equiv_refl;
-try reflexivity.
+try rewrite !andb_true_r;
+try reflexivity;
+rewrite !Compare_dec.leb_correct;
+lia.
 Qed.
-
-Lemma not_weak_equiv_eqb :
-    forall (A1 A2 : formula),
-        weak_formula A2 = false ->
-            form_equiv A1 A2 = form_eqb A1 A2.
-Proof.
-induction A1;
-destruct A2;
-intros WF;
-try apply orb_false_elim in WF as [WF1 WF2];
-unfold form_equiv, form_eqb;
-fold form_equiv form_eqb;
-try rewrite IHA1;
-try rewrite IHA1_1, IHA1_2;
-try apply WF;
-try apply WF1;
-try apply WF2;
-try reflexivity.
-rewrite WF1, WF2, !orb_false_l.
-reflexivity.
-Qed.
-
-Lemma equiv_trans :
-    forall (A1 A2 A3 : formula),
-        form_equiv A1 A2 = true ->
-            form_equiv A2 A3 = true ->
-                form_equiv A1 A3 = true.
-Proof.
-induction A1;
-destruct A2, A3;
-intros EQ1 EQ2;
-try inversion EQ1 as [EQ1'];
-try inversion EQ2 as [EQ2'];
-try rewrite EQ1'.
-- reflexivity.
-- unfold form_equiv;
-  fold form_equiv.
-  case (nat_eqb i1 0) eqn:EQB1;
-  try apply nat_eqb_eq in EQB1;
-  subst;
-  case (nat_eqb i2 0) eqn:EQB2;
-  try apply nat_eqb_eq in EQB2;
-  subst;
-  case (nat_eqb i3 0) eqn:EQB3;
-  try apply nat_eqb_eq in EQB3;
-  subst;
-  case (nat_eqb i4 0) eqn:EQB4;
-  try apply nat_eqb_eq in EQB4;
-  subst;
-  try rewrite !orb_false_l in *;
-  try rewrite !orb_false_r in *;
-  try rewrite !orb_true_l in *;
-  try rewrite !orb_true_r in *;
-  try rewrite !andb_true_l in *;
-  try rewrite !andb_true_r in *;
-  try apply and_bool_prop in EQ1' as [EQ1_1 EQ1_2];
-  try apply and_bool_prop in EQ2' as [EQ2_1 EQ2_2];
-  try apply nat_eqb_eq in EQ1';
-  try apply nat_eqb_eq in EQ2';
-  try apply nat_eqb_eq in EQ1_1;
-  try apply nat_eqb_eq in EQ1_2;
-  try apply nat_eqb_eq in EQ2_1;
-  try apply nat_eqb_eq in EQ2_2;
-  subst;
-  try rewrite !nat_eqb_refl in *;
-  try reflexivity;
-  try discriminate.
-- unfold form_equiv;
-  fold form_equiv.
-  apply and_bool_prop in EQ1 as [EQ1_1 EQ1_2].
-  apply and_bool_prop in EQ2 as [EQ2_1 EQ2_2].
-  rewrite (IHA1_1 _ _ EQ1_1 EQ2_1).
-  rewrite (IHA1_2 _ _ EQ1_2 EQ2_2).
-  reflexivity.
-- unfold form_equiv;
-  fold form_equiv.
-  apply and_bool_prop in EQ1 as [EQ1_1 EQ1_2].
-  apply and_bool_prop in EQ2 as [EQ2_1 EQ2_2].
-  apply nat_eqb_eq in EQ1_1, EQ2_1.
-  subst.
-  rewrite (IHA1 _ _ EQ1_2 EQ2_2).
-  rewrite nat_eqb_refl.
-  reflexivity.
-- unfold form_equiv;
-  fold form_equiv.
-  apply and_bool_prop in EQ1 as [EQ1_1 EQ1_2].
-  apply and_bool_prop in EQ2 as [EQ2_1 EQ2_2].
-  apply and_bool_prop in EQ1_1 as [EQN1 EQN2], EQ2_1 as [EQN3 EQN4].
-  apply nat_eqb_eq in EQN1, EQN2, EQN3, EQN4.
-  subst.
-  rewrite (IHA1 _ _ EQ1_2 EQ2_2).
-  rewrite !nat_eqb_refl.
-  reflexivity.
-- pose proof (prd_eqb_type _ _ EQ1') as [EQN1 EQV1].
-  pose proof (prd_eqb_type _ _ EQ2') as [EQN2 EQV2].
-  apply nat_eqb_eq in EQN1, EQN2.
-  subst.
-  apply nvec_eqb_eq in EQV1, EQV2.
-  subst.
-  apply prd_eqb_eq in EQ1', EQ2'.
-  subst.
-  apply EQ2.
-Qed.
+*)
 
 (*
-Lemma equiv_anti_trans :
-    forall (A1 A2 A3 : formula),
-        weak_formula A3 = false ->
-            form_equiv A1 A2 = true ->
-                form_equiv A2 A3 = false ->
-                    form_equiv A1 A3 = false.
+Lemma form_equiv_succ_form :
+    forall (phi : formula) (d v1 v2 : nat),
+        d < (S v1) -> d < (S v2)  -> 
+        form_equiv (substitution_depth phi 0 (S v1) (S v2)) phi d = true ->
+            form_equiv (substitution_depth phi 1 (S v1) (S v2)) phi (S d) = true.
 Proof.
-induction A1;
-destruct A2, A3;
-intros WF EQ1 EQ2;
-try inversion EQ1 as [EQ1'];
-try inversion EQ2 as [EQ2'];
-try rewrite EQ1';
-try rewrite EQ2';
+induction phi;
+intros d v1 v2 LT1 LT2 EQ;
+unfold substitution_depth in *;
+fold substitution_depth in *;
+unfold form_equiv in *;
+fold form_equiv in *;
 try reflexivity.
-- unfold form_equiv;
-  fold form_equiv.
-  case (nat_eqb i1 0) eqn:EQB1;
-  try apply nat_eqb_eq in EQB1;
+- case (nat_eqb i (S v1)) eqn:EQ1;
+  case (nat_eqb i0 (S v1)) eqn:EQ2;
+  try apply nat_eqb_eq in EQ1;
+  try apply nat_eqb_eq in EQ2;
   subst;
-  case (nat_eqb i2 0) eqn:EQB2;
-  try apply nat_eqb_eq in EQB2;
+  unfold form_equiv in *;
+  fold form_equiv in *;
+  try rewrite !nat_eqb_refl;
+  try rewrite !orb_true_l;
+  try rewrite andb_true_l;
+  try rewrite andb_true_r;
+  try rewrite !Compare_dec.leb_correct;
+  try lia.
+- apply and_bool_prop in EQ as [EQ1 EQ2].
+  rewrite IHphi1, IHphi2;
+  try assumption;
+  try reflexivity.
+- unfold nat_ltb, Nat.leb in EQ.
+- repeat apply and_bool_prop in EQ as [EQ ?EQ].
+  rewrite !nat_eqb_refl, !andb_true_l.
+  apply IHphi;
+  assumption.
+- apply EQ.
+Admitted.
+
+Lemma free_sub_means_equiv_other :
+    forall (phi : formula) (v1 v2 : ivar) (d2 : nat),
+        d2 < v1 ->
+          d2 < v2 ->
+            form_equiv (substitution_depth phi 0 v1 v2) phi d2 = true.
+Proof.
+induction phi;
+intros v1 v2 d LT1 LT2;
+unfold substitution_depth;
+fold substitution_depth;
+unfold form_depth;
+fold form_depth;
+unfold form_equiv;
+fold form_equiv;
+try rewrite !nat_eqb_refl;
+try rewrite prd_eqb_refl;
+try rewrite IHphi;
+try rewrite IHphi1;
+try rewrite IHphi2;
+try reflexivity;
+unfold form_depth in *;
+fold form_depth in *;
+try lia.
+case (nat_eqb i v1) eqn:EQ1;
+case (nat_eqb i0 v1) eqn:EQ2;
+try apply nat_eqb_eq in EQ1;
+try apply nat_eqb_eq in EQ2;
+subst;
+unfold form_equiv;
+fold form_equiv;
+try rewrite !nat_eqb_refl;
+try rewrite plus_O_n in *;
+try rewrite (nat_lt_ltb _ _ LT1);
+try rewrite (nat_lt_ltb _ _ LT2);
+try rewrite !orb_true_l;
+try rewrite !orb_true_r;
+try reflexivity;
+try rewrite !Compare_dec.leb_correct;
+try lia.
+
+destruct v1.
+inversion LT1.
+destruct v2.
+inversion LT2.
+unfold nat_ltb, Nat.leb.
+unfold form_equiv;
+fold form_equiv.
+pose proof (IHphi (S v1) (S v2) d LT1 LT2).
+apply form_equiv_succ_form in H.
+apply H.
+all : lia.
+Qed.
+*)
+
+(*
+Lemma form_equiv_sym :
+    forall (phi1 phi2 : formula) (d : nat),
+        form_equiv phi1 phi2 d = form_equiv phi2 phi1 d.
+Proof.
+induction phi1;
+destruct phi2;
+intros d;
+unfold form_equiv;
+fold form_equiv;
+try rewrite (nat_eqb_symm i i1);
+try rewrite (nat_eqb_symm i0 i2);
+try rewrite (nat_eqb_symm o o1);
+try rewrite (nat_eqb_symm o0 o2);
+try rewrite (andb_comm (nat_leb _ i1));
+try rewrite (andb_comm (nat_leb _ i2));
+try rewrite prd_eqb_sym;
+try rewrite IHphi1;
+try rewrite IHphi1_1, IHphi1_2;
+try reflexivity.
+admit.
+Admitted.
+*)
+
+(*
+Lemma form_equiv_trans :
+    forall (phi1 phi2 phi3 : formula) (d : nat),
+        form_equiv phi1 phi2 d = true ->
+            form_equiv phi2 phi3 d = true ->
+                form_equiv phi1 phi3 d = true.
+Proof.
+induction phi1;
+destruct phi2, phi3;
+intros d EQ1 EQ2;
+try reflexivity;
+inversion EQ1 as [EQ1'];
+try rewrite EQ1';
+inversion EQ2 as [EQ2'];
+try rewrite EQ2';
+unfold form_equiv;
+fold form_equiv;
+try case (nat_eqb i i0) eqn:EQB1;
+try rewrite EQ1' in EQ2';
+try apply and_bool_prop in EQ1' as [EQ3 EQ4];
+try apply and_bool_prop in EQ2' as [EQ5 EQ6].
+- apply EQ2'.
+- case (nat_eqb i1 i2) eqn:EQB2.
+  apply nat_eqb_eq in EQB2,EQ2'.
   subst.
-  case (nat_eqb i3 0) eqn:EQB3;
-  try apply nat_eqb_eq in EQB3;
+  apply or_bool_prop in EQ3 as [EQ3 | LT1];
+  apply or_bool_prop in EQ4 as [EQ4 | LT3];
+  try apply nat_eqb_eq in EQ3;
+  try apply nat_eqb_eq in EQ4;
   subst;
-  case (nat_eqb i4 0) eqn:EQB4;
-  try apply nat_eqb_eq in EQB4;
+  try apply and_bool_prop in LT1 as [LT1 LT2];
+  try apply and_bool_prop in LT3 as [LT3 LT4];
+  try rewrite nat_eqb_refl in EQB1;
+  try inversion EQB1;
+  try rewrite LT1;
+  try rewrite LT2;
+  try rewrite LT3;
+  try rewrite LT4.
+  try rewrite orb_true_l.
+  admit.
+  admit.
+  
+  
+  apply or_bool_prop in EQ3 as [EQ3 | LT1];
+  apply or_bool_prop in EQ4 as [EQ4 | LT3];
+  apply or_bool_prop in EQ5 as [EQ5 | LT5];
+  apply or_bool_prop in EQ6 as [EQ6 | LT7];
+  try apply nat_eqb_eq in EQ3;
+  try apply nat_eqb_eq in EQ4;
+  try apply nat_eqb_eq in EQ5;
+  try apply nat_eqb_eq in EQ6;
+  try apply and_bool_prop in LT1 as [LT1 LT2];
+  try apply and_bool_prop in LT3 as [LT3 LT4];
+  try apply and_bool_prop in LT5 as [LT5 LT6];
+  try apply and_bool_prop in LT7 as [LT7 LT8];
   subst;
-  try rewrite !orb_false_l in *;
-  try rewrite !orb_false_r in *;
-  try rewrite !orb_true_l in *;
-  try rewrite !orb_true_r in *;
-  try rewrite !andb_true_l in *;
-  try rewrite !andb_true_r in *;
-  try apply and_bool_prop in EQ1' as [EQ1_1 EQ1_2];
-  try apply and_bool_prop in EQ2' as [EQ2_1 EQ2_2];
-  try apply nat_eqb_eq in EQ1';
-  try apply nat_eqb_eq in EQ2';
-  try apply nat_eqb_eq in EQ1_1;
-  try apply nat_eqb_eq in EQ1_2;
-  try apply nat_eqb_eq in EQ2_1;
-  try apply nat_eqb_eq in EQ2_2;
-  subst;
-  try rewrite !nat_eqb_refl in *;
-  try reflexivity;
-  try discriminate.
-- unfold form_equiv;
-  fold form_equiv.
-  apply orb_false_elim in WF as [WF1 WF2].
-  apply and_bool_prop in EQ1 as [EQ1_1 EQ1_2].
-  apply andb_false_elim in EQ2 as [EQ2_1 | EQ2_2].
-  rewrite (IHA1_1 _ _ WF1 EQ1_1 EQ2_1).
-  apply andb_false_l.
-  rewrite (IHA1_2 _ _ WF2 EQ1_2 EQ2_2).
-  apply andb_false_r.
-- unfold form_equiv;
-  fold form_equiv.
-  apply and_bool_prop in EQ1 as [EQ1_1 EQ1_2].
-  apply andb_false_elim in EQ2 as [EQ2_1 | EQ2_2].
-  apply nat_eqb_eq in EQ1_1.
+  try rewrite !nat_eqb_refl;
+  try rewrite LT1;
+  try rewrite LT2;
+  try rewrite LT3;
+  try rewrite LT4;
+  try rewrite LT5;
+  try rewrite LT6;
+  try rewrite LT7;
+  try rewrite LT8;
+  try rewrite !orb_true_l;
+  try rewrite !orb_true_r;
+  try reflexivity.
+- rewrite (IHphi1_1 _ _ _ EQ3 EQ5), (IHphi1_2 _ _ _ EQ4 EQ6).
+  reflexivity.
+- apply (IHphi1 _ _ _ EQ1' EQ2').
+- apply and_bool_prop in EQ3 as [EQ3 EQ7].
+  apply and_bool_prop in EQ5 as [EQ5 EQ8].
+  apply nat_eqb_eq in EQ3,EQ5,EQ7,EQ8.
   subst.
-  rewrite EQ2_1.
-  apply andb_false_l.
-  unfold weak_formula in WF.
-  rewrite (IHA1 _ _ WF EQ1_2 EQ2_2).
-  apply andb_false_r.
-- unfold form_equiv;
-  fold form_equiv.
-  apply and_bool_prop in EQ1 as [EQ1_1 EQ1_2].
-  apply and_bool_prop in EQ1_1 as [EQN1 EQN2].
+  rewrite !nat_eqb_refl.
+  apply (IHphi1 _ _ _ EQ4 EQ6).
+- pose proof (prd_eqb_type _ _ EQ1') as EQN1.
+  pose proof (prd_eqb_type _ _ EQ2') as EQN2.
   apply nat_eqb_eq in EQN1,EQN2.
   subst.
-  apply andb_false_elim in EQ2 as [EQ2_1 | EQ2_2].
-  rewrite EQ2_1.
-  apply andb_false_l.
-  unfold weak_formula in WF.
-  rewrite (IHA1 _ _ WF EQ1_2 EQ2_2).
-  apply andb_false_r.
-- pose proof (prd_eqb_type _ _ EQ1') as [EQN1 EQV1].
-  apply nat_eqb_eq in EQN1.
+  apply prd_eqb_eq in EQ1',EQ2'.
   subst.
-  apply nvec_eqb_eq in EQV1.
-  subst.
-  apply prd_eqb_eq in EQ1'.
-  subst.
-  apply EQ2.
-Admitted.
-*)
-
-Lemma not_weak_sub0_not_weak :
-    forall (phi : formula) (v : ivar),
-        weak_formula phi = false ->
-            weak_formula (substitution phi 0 (S v)) = false.
-Proof.
-induction phi;
-intros v WF;
-unfold substitution;
-fold substitution;
-unfold weak_formula in *;
-fold weak_formula in *;
-try reflexivity.
-apply orb_false_elim in WF as [WF1 WF2].
-rewrite WF1, WF2.
-unfold weak_formula.
-rewrite WF1, WF2.
-reflexivity.
-apply orb_false_elim in WF as [WF1 WF2].
-rewrite (IHphi1 _ WF1), (IHphi2 _ WF2).
-reflexivity.
-case (nat_eqb i 0) eqn:EQB.
-apply WF.
-apply (IHphi _ WF).
-apply (IHphi _ WF).
-Qed.
-
-Lemma not_weak_sub0_triv :
-    forall (phi : formula) (v : ivar),
-        weak_formula phi = false ->
-            (substitution phi 0 v) = phi.
-Proof.
-induction phi;
-intros v WF;
-unfold substitution;
-fold substitution;
-unfold weak_formula in *;
-fold weak_formula in *;
-try reflexivity.
-apply orb_false_elim in WF as [WF1 WF2].
-rewrite WF1, WF2.
-reflexivity.
-apply orb_false_elim in WF as [WF1 WF2].
-rewrite (IHphi1 _ WF1), (IHphi2 _ WF2).
-reflexivity.
-case (nat_eqb i 0) eqn:EQB.
-reflexivity.
-rewrite (IHphi _ WF).
-reflexivity.
-rewrite (IHphi _ WF).
-reflexivity.
-Qed.
-
-Lemma no_bind_sub0_not_weak :
-    forall (phi : formula) (v : ivar),
-        binds0 phi = false -> 
-            weak_formula (substitution phi 0 (S v)) = false.
-Proof.
-induction phi;
-intros v BO;
-unfold substitution;
-fold substitution;
-unfold binds0;
-fold binds0;
-unfold weak_formula;
-fold weak_formula.
-- reflexivity.
-- case (nat_eqb i 0) eqn:EQB1;
-  case (nat_eqb i0 0) eqn:EQB2;
-  unfold weak_formula;
-  try rewrite EQB1;
-  try rewrite EQB2;
-  reflexivity.
-- apply orb_false_elim in BO as [BO1 BO2].
-  rewrite (IHphi1 _ BO1), (IHphi2 _ BO2).
-  reflexivity.
-- apply orb_false_elim in BO as [BO1 BO2].
-  case (nat_eqb i 0) eqn:EQ.
-  apply BO1.
-  apply (IHphi _ BO2).  
-- apply (IHphi _ BO).
-- reflexivity.
-Qed.
-
-Lemma sub0_not_weak_no_bind :
-    forall (phi : formula) (v : ivar),
-        weak_formula (substitution phi 0 (S v)) = false ->
-            binds0 phi = false.
-Proof.
-induction phi;
-intros v WF;
-unfold substitution in *;
-fold substitution in *;
-unfold binds0 in *;
-fold binds0 in *;
-unfold weak_formula in *;
-fold weak_formula in *;
-try reflexivity.
-- apply orb_false_elim in WF as [WF1 WF2].
-  rewrite (IHphi1 _ WF1), (IHphi2 _ WF2).
-  reflexivity.
-- case (nat_eqb i 0) eqn:EQ.
-  + unfold weak_formula in WF;
-    fold weak_formula in WF.
-    rewrite WF.
-    apply (IHphi 0 (not_weak_sub0_not_weak _ _ WF)).
-  + apply (IHphi _ WF).
-- apply (IHphi _ WF).
-Qed.
-
-Lemma equiv_test :
-    forall (phi A : formula) (v1 v2 : ivar) ,
-        formula_sub (substitution phi 0 v1) phi A true = formula_sub (substitution phi 0 v2) phi A true.
-Proof.
-intros phi A v1 v2.
-unfold formula_sub.
-rewrite !form_equiv_sub0.
-reflexivity.
-Qed.
-
-Lemma form_sub_sub0_comm :
-    forall (phi A1 A2 : formula) (v : ivar) (b : bool),
-        weak_formula A1 = false ->
-            weak_formula A2 = false ->
-                (substitution (formula_sub phi A1 A2 b) 0 v) = formula_sub (substitution phi 0 v) A1 A2 b.
-Proof.
-intros phi A1 A2 v b WF1 WF2.
-unfold formula_sub.
-case (form_equiv (substitution phi 0 v) A1) eqn:EQF1;
-case (form_equiv phi A1) eqn:EQF2.
-1,2 : destruct b.
-all : try reflexivity.
-- apply not_weak_sub0_triv, WF2.
-
-- rewrite (not_weak_equiv_eqb _ _ WF1) in EQF1. admit.
-
-- rewrite (equiv_trans _ _ _ (form_equiv_sub0 _ _) EQF2) in EQF1.
-  inversion EQF1.
-Qed.
-  
-induction phi;
-intros A1 A2 v b WF1 WF2;
-unfold formula_sub;
-unfold substitution;
-fold substitution.
-- case (form_equiv fal A1) eqn:EQF.
-  destruct b.
-  apply not_weak_sub0_triv, WF2.
-  reflexivity.
-  reflexivity.
-- admit.
-- case (form_equiv _ A1) eqn:EQF.
-  destruct A1;
-  inversion EQF.
-  apply and_bool_prop in H0 as [EQF1 EQF2].
-  unfold form_equiv;
-  fold form_equiv.
-  rewrite (equiv_trans _ _ _ (form_equiv_sub0 _ _) EQF1).
-  rewrite (equiv_trans _ _ _ (form_equiv_sub0 _ _) EQF2).
-  unfold "&&".
-  destruct b.
-  apply not_weak_sub0_triv, WF2.
-  reflexivity.
-  unfold
-
-  admit.
-- admit.
-- admit.
-- admit.
-
-  
-Admitted.
-
-Lemma not_weak_sub_not_weak : 
-    forall (phi A1 A2 : formula),
-        weak_formula phi = false ->
-            weak_formula A2 = false ->
-                forall (b : bool),
-                    weak_formula (formula_sub phi A1 A2 b) = false.
-Proof.
-induction phi;
-intros A1 A2 WF1 WF2 b;
-unfold formula_sub;
-case (form_equiv _ A1) eqn:EQF;
-destruct b;
-try apply WF1;
-apply WF2.
-Qed.
-
-(*
-Lemma equiv_test :
-    forall (phi A : formula) (v1 v2 : ivar) ,
-        formula_sub (substitution phi 0 v1) phi A true = formula_sub (substitution phi 0 v2) phi A true.
-Proof.
-intros phi A v1 v2.
-unfold formula_sub.
-rewrite !form_equiv_sub0.
-reflexivity.
+  apply prd_eqb_refl.
 Qed.
 *)
 
-Fixpoint batch_sub_fit (gamma : list formula) (A1 A2 : formula) (S : subst_ind) : list formula :=
+Definition formula_sub (phi A1 A2 : formula) (d : nat) (b : bool) : formula :=
+match form_equiv phi A1 d, b with
+| true, true => A2
+| _, _ => phi
+end.
+
+Fixpoint batch_sub_fit (gamma : list formula) (A1 A2 : formula) (d : nat) (S : subst_ind) : list formula :=
 match gamma, S with
-| phi :: gamma', b :: S' => (formula_sub phi A1 A2 b) :: batch_sub_fit gamma' A1 A2 S'
+| phi :: gamma', b :: S' => (formula_sub phi A1 A2 d b) :: batch_sub_fit gamma' A1 A2 d S'
 | _ , _ => gamma
 end.
 
-Definition batch_sub (gamma : list formula) (A1 A2 : formula) (S : subst_ind) : list formula :=
+Definition batch_sub (gamma : list formula) (A1 A2 : formula) (d : nat) (S : subst_ind) : list formula :=
 match nat_eqb (length gamma) (length S) with
 | false => gamma
-| true => batch_sub_fit gamma A1 A2 S
+| true => batch_sub_fit gamma A1 A2 d S
 end.
 
-Lemma formula_sub_false {phi A1 A2 : formula} : formula_sub phi A1 A2 false = phi.
-Proof. unfold formula_sub. case (form_equiv phi A1); reflexivity. Qed.
+Lemma formula_sub_false {phi A1 A2 : formula} :
+    forall (d : nat),
+        formula_sub phi A1 A2 d false = phi.
+Proof. intros d. unfold formula_sub. case (form_equiv phi A1); reflexivity. Qed.
 
 Lemma batch_sub_nil :
-    forall (gamma : list formula) (A1 A2 : formula),
-        batch_sub_fit gamma A1 A2 [] = gamma.
+    forall (gamma : list formula) (A1 A2 : formula) (d : nat),
+        batch_sub_fit gamma A1 A2 d [] = gamma.
 Proof. induction gamma; reflexivity. Qed.
 
 Lemma batch_sub_fit_true :
-    forall {gamma : list formula} {A1 A2 : formula} {S : subst_ind},
+    forall {gamma : list formula} {A1 A2 : formula} {d : nat} {S : subst_ind},
         nat_eqb (length gamma) (length S) = true ->
-            batch_sub_fit gamma A1 A2 S = batch_sub gamma A1 A2 S.
-Proof. intros gamma A1 A2 S EQ. unfold batch_sub. rewrite EQ. reflexivity. Qed.
+            batch_sub_fit gamma A1 A2 d S = batch_sub gamma A1 A2 d S.
+Proof. intros gamma A1 A2 d S EQ. unfold batch_sub. rewrite EQ. reflexivity. Qed.
 
 Lemma batch_sub_single :
-    forall (phi : formula) (A1 A2 : formula) (b : bool),
-            batch_sub [phi] A1 A2 [b] = [formula_sub phi A1 A2 b].
+    forall (phi : formula) (A1 A2 : formula) (d : nat) (b : bool),
+            batch_sub [phi] A1 A2 d [b] = [formula_sub phi A1 A2 d b].
 Proof. reflexivity. Qed.
 
 Lemma batch_sub_false_head :
-    forall (phi : formula) (gamma : list formula) (A1 A2 : formula) (S : subst_ind),
-            batch_sub (phi :: gamma) A1 A2 (false :: S) = phi :: batch_sub gamma A1 A2 S.
+    forall (phi : formula) (gamma : list formula) (A1 A2 : formula) (d : nat) (S : subst_ind),
+            batch_sub (phi :: gamma) A1 A2 d (false :: S) = phi :: batch_sub gamma A1 A2 d S.
 Proof.
-intros phi gamma A1 A2 S.
+intros phi gamma A1 A2 d S.
 unfold batch_sub, length, nat_eqb.
 fold nat_eqb (@length formula) (@length bool).
 case (nat_eqb (length gamma) (length S));
@@ -545,13 +407,13 @@ reflexivity.
 Qed.
 
 Lemma batch_app_split :
-    forall (gamma1 gamma2 : list formula) (A1 A2 : formula) (S1 S2 : subst_ind),
+    forall (gamma1 gamma2 : list formula) (A1 A2 : formula) (d : nat) (S1 S2 : subst_ind),
         length gamma1 = length S1 ->
             length gamma2 = length S2 ->
-                batch_sub (gamma1 ++ gamma2) A1 A2 (S1 ++ S2) = batch_sub gamma1 A1 A2 S1 ++ batch_sub gamma2 A1 A2 S2.
+                batch_sub (gamma1 ++ gamma2) A1 A2 d (S1 ++ S2) = batch_sub gamma1 A1 A2 d S1 ++ batch_sub gamma2 A1 A2 d S2.
 Proof.
 induction gamma1;
-intros gamma2 A1 A2 S1 S2 EQ1 EQ2;
+intros gamma2 A1 A2 d S1 S2 EQ1 EQ2;
 destruct S1;
 inversion EQ1 as [EQ].
 reflexivity.
@@ -569,11 +431,11 @@ all : try rewrite EQ;
 Qed.
 
 Lemma batch_bury_comm_aux :
-    forall (n : nat) (LF : list formula) (S : subst_ind) (A1 A2 : formula),
-        bury (batch_sub LF A1 A2 S) n = batch_sub (bury LF n) A1 A2 (bury S n).
+    forall (n : nat) (LF : list formula) (d : nat) (S : subst_ind) (A1 A2 : formula),
+        bury (batch_sub LF A1 A2 d S) n = batch_sub (bury LF n) A1 A2 d (bury S n).
 Proof.
 induction n;
-intros LF LS A v;
+intros LF d LS A v;
 unfold batch_sub;
 rewrite !bury_length;
 case (nat_eqb (length LF) (length LS)) eqn:EQ;
@@ -605,21 +467,21 @@ apply EQ.
 Qed.
 
 Lemma batch_bury_comm :
-    forall (LF : list formula) (LS : subst_ind) (n : nat) (A1 A2 : formula),
-        bury (batch_sub LF A1 A2 (unbury LS n)) n = batch_sub (bury LF n) A1 A2 LS.
+    forall (LF : list formula) (LS : subst_ind) (n d : nat) (A1 A2 : formula),
+        bury (batch_sub LF A1 A2 d (unbury LS n)) n = batch_sub (bury LF n) A1 A2 d LS.
 Proof.
-intros LF LS n A1 A2.
+intros LF LS n d A1 A2.
 rewrite <- (@bury_unbury _ LS n) at 2.
 apply batch_bury_comm_aux.
 Qed.
 
 Lemma batch_sub_app {A1 A2 : formula} :
-    forall (L1 L2 : list formula) (S : subst_ind),
+    forall (L1 L2 : list formula) (d : nat) (S : subst_ind),
         length (L1 ++ L2) = length S ->
-            batch_sub (L1 ++ L2) A1 A2 S = batch_sub L1 A1 A2 (firstn (length L1) S) ++ batch_sub L2 A1 A2 (skipn (length L1) S).
+            batch_sub (L1 ++ L2) A1 A2 d S = batch_sub L1 A1 A2 d (firstn (length L1) S) ++ batch_sub L2 A1 A2 d (skipn (length L1) S).
 Proof.
 induction L1;
-intros L2 S EQ.
+intros L2 d S EQ.
 rewrite !app_nil_l in *.
 reflexivity.
 destruct S.
@@ -634,7 +496,7 @@ unfold firstn, skipn;
 fold (@firstn bool) (@skipn bool).
 unfold batch_sub_fit;
 fold batch_sub_fit.
-rewrite !batch_sub_fit_true, (IHL1 _ _ EQ).
+rewrite !batch_sub_fit_true, (IHL1 _ _ _ EQ).
 reflexivity.
 rewrite skipn_length, <- EQ, app_length, minus_n_plus_m.
 apply nat_eqb_refl.
@@ -647,12 +509,12 @@ apply PeanoNat.Nat.le_add_r.
 Qed.
 
 Lemma batch_sub_is_map_combine : 
-    forall L A1 A2 S,
+    forall (L : list formula) (A1 A2 : formula) (d : nat) (S : subst_ind),
         length L = length S ->
-            batch_sub L A1 A2 S = (map (fun PAIR => formula_sub (fst PAIR) A1 A2 (snd (PAIR))) (combine L S)).
+            batch_sub L A1 A2 d S = (map (fun PAIR => formula_sub (fst PAIR) A1 A2 d (snd (PAIR))) (combine L S)).
 Proof.
 induction L;
-intros A1 A2 S EQ;
+intros A1 A2 d S EQ;
 unfold combine, batch_sub, batch_sub_fit, map;
 fold batch_sub_fit (@combine formula bool);
 rewrite EQ, nat_eqb_refl.
@@ -670,13 +532,13 @@ Qed.
 
 (*
 Lemma map_batch_sub : 
-    forall (gamma : list formula) (A1 A2 : formula) (S : subst_ind) (F : formula -> formula),
+    forall (gamma : list formula) (A1 A2 : formula) (d : nat) (S : subst_ind) (F : formula -> formula),
         (forall (phi1 phi2 : formula),
             phi1 = phi2 <-> F phi1 = F phi2) ->
-            map F (batch_sub gamma A1 A2 S) = batch_sub (map F gamma) (F A1) (F A2) S.
+            map F (batch_sub gamma A1 A2 d S) = batch_sub (map F gamma) (F A1) (F A2) d S.
 Proof.
 induction gamma;
-intros A1 A2 S F INJ;
+intros A1 A2 d S F INJ;
 unfold batch_sub, batch_sub_fit.
 - destruct S;
   rewrite map_length;
@@ -698,14 +560,13 @@ unfold batch_sub, batch_sub_fit.
     rewrite !batch_sub_fit_true.
     rewrite IHgamma.
     unfold formula_sub.
-    case (form_equiv a A1) eqn:EQF;
+    case (form_equiv a A1 d) eqn:EQF;
     destruct b;
     try apply form_eqb_eq in EQF;
     subst;
-    try rewrite !form_equiv_refl;
+    try rewrite !form_eqb_refl;
     try reflexivity.
-    * case (form_equiv (F a) (F A1)) eqn:FAL.
-      reflexivity.
+    * case (form_eqb (F a) (F A1)) eqn:FAL.
       apply form_eqb_eq, INJ in FAL.
       subst.
       rewrite form_eqb_refl in EQF.
@@ -719,15 +580,16 @@ unfold batch_sub, batch_sub_fit.
     * apply EQB.
   + reflexivity.
 Qed.
+*)
 
 Lemma batch_sub_sublist :
-    forall (L1 L2 : list formula) (A1 A2 : formula) (S : subst_ind),
+    forall (L1 L2 : list formula) (A1 A2 : formula) (d : nat) (S : subst_ind),
         sublist form_eq_dec L1 L2 = true ->
             length L2 = length S ->
-                sublist form_eq_dec (batch_sub L1 A1 A2 (list_filter S ((sublist_filter form_eq_dec L1 L2)))) (batch_sub L2 A1 A2 S) = true.
+                sublist form_eq_dec (batch_sub L1 A1 A2 d (list_filter S ((sublist_filter form_eq_dec L1 L2)))) (batch_sub L2 A1 A2 d S) = true.
 Proof.
 induction L1;
-intros L2 A1 A2 S SL EQ.
+intros L2 A1 A2 d S SL EQ.
 unfold batch_sub, batch_sub_fit.
 fold batch_sub_fit.
 rewrite EQ at 1.
@@ -741,12 +603,12 @@ assert (Nat.min (length L3) (length S) = length L3) as EQ'.
   apply min_l, PeanoNat.Nat.le_add_r. }
 
 rewrite (sublist_cons_split_filter form_eq_dec _ _ _ _ SL NIN).
-rewrite (batch_sub_app _ _ _ EQ).
+rewrite (batch_sub_app _ _ _ _ EQ).
 rewrite <- (firstn_skipn (length L3) S) at 1.
 rewrite list_filter_app.
 - rewrite firstn_length.
   rewrite EQ'.
-  rewrite plus_n_O at 2 5.
+  rewrite (plus_n_O (length L3)) at 2 5.
   rewrite <- (repeat_length false (length L3)) at 2 5.
   rewrite firstn_app_2.
   rewrite skipn_app2.
@@ -781,7 +643,7 @@ rewrite list_filter_app.
   fold @sublist.
   rewrite !batch_sub_fit_true.
   + case form_eq_dec as [_ | FAL].
-    apply (IHL1 _ _ _ _ SL' (eq_sym LEN')).
+    apply (IHL1 _ _ _ _ _ SL' (eq_sym LEN')).
     contradiction (FAL eq_refl).
   + rewrite LEN'.
     apply nat_eqb_refl.
@@ -1103,5 +965,4 @@ rewrite formula_sub_ind_lor.
 - rewrite FS.
   apply non_target_fit.
 Qed.
-*)
 *)
