theories/Maths/naturals.v
@@ -6,6 +6,7 @@ Open Scope bool_scope.
 
 Notation nat_eqb := Nat.eqb.
 Notation nat_ltb := Nat.ltb.
+Notation nat_leb := Nat.leb.
 Notation nat_eq_dec := PeanoNat.Nat.eq_dec.
 
 Lemma nat_eqb_refl :
